@prefix exp: <http://purl.imsglobal.org/vocab/caliper/v1/core#> .
@prefix xsd: <http://www.w3.org/2001/XMLSchema#> .
@prefix owl: <http://www.w3.org/2002/07/owl#> .
@prefix rdf: <http://www.w3.org/1999/02/22-rdf-syntax-ns#> .
@prefix rdfs: <http://www.w3.org/2000/01/rdf-schema#> .
@prefix bind: <http://purl.org/semantictools/v1/vocab/bind#> .

<http://purl.imsglobal.org/vocab/caliper/v1/core#> a owl:Ontology  ;
  rdfs:label "Caliper Core" ;
  a bind:TargetNamespace ;
  bind:suggestedPrefix "exp" .

exp:Activity rdf:type owl:Class;
  rdfs:subClassOf 
  [ a owl:Restriction ;
    owl:onProperty      exp:activity_id;
    owl:minCardinality  1;
    rdfs:comment "The unique ID for the activity as used by the tool provider."
  ] ; 
  rdfs:comment "A resource that a person may experience such as a video or an assessment.  This entity represents the resource itself, not the person's engagement with the resource." .

exp:activity_id rdf:type owl:FunctionalProperty ;
  rdfs:domain exp:Activity ;
  rdfs:range xsd:normalizedString ;
  rdfs:comment "The unique ID for the activity as used by the tool provider." .

exp:activityTemplate rdf:type owl:FunctionalProperty ;
  rdfs:domain exp:Activity ;
  rdfs:range exp:Activity .

