@prefix lisp: <http://localhost/purl.imsglobal.org/vocab/lis/v2/pm#> .
@prefix xsd: <http://www.w3.org/2001/XMLSchema#> .
@prefix schema: <http://schema.org/> .
@prefix lism: <http://localhost/purl.imsglobal.org/vocab/lis/v2/mm#> .
@prefix org: <http://www.w3.org/ns/org#> .
@prefix owl: <http://www.w3.org/2002/07/owl#> .
@prefix rdf: <http://www.w3.org/1999/02/22-rdf-syntax-ns#> .
@prefix rdfs: <http://www.w3.org/2000/01/rdf-schema#> .
@prefix bind: <http://purl.org/semantictools/v1/vocab/bind#> .
@prefix vann: <http://purl.org/vocab/vann#> .

<http://localhost/purl.imsglobal.org/vocab/lis/v2/pm#> a owl:Ontology  ;
  rdfs:label "LIS Person Management" ;
  a bind:TargetNamespace ;
  bind:suggestedPrefix "lisp" .

lisp:LISPerson rdf:type owl:Class ;
  rdfs:subClassOf schema:Person ,
  [ a owl:Restriction ;
    owl:onProperty      lisp:user_id;
    owl:minCardinality  1;
    owl:maxCardinality  1;
    rdfs:comment "A unique identifier for the person."
  ] ,
  [ a owl:Restriction ;
    owl:onProperty      lisp:sourcedId;
    owl:maxCardinality  1;
    rdfs:comment "A unique identifier for the person as provisioned by an external system such as an SIS."
  ] ,
  [ a owl:Restriction ;
    owl:onProperty      lisp:email;
    owl:maxCardinality  1;
    rdfs:comment "The primary email address for the person."
  ] ,
  [ a owl:Restriction ;
    owl:onProperty      lisp:resultSourcedId;
    owl:maxCardinality  1;
    rdfs:comment "The person's LIS Result Identifier (if any) associated with a launch from the organization.  This will normally only have a value if the organization represents a resource link, though could also reflect a course-level launch."
  ] ,
  [ a owl:Restriction ;
    owl:onProperty      org:hasMembership;
    owl:allValuesFrom  lism:LISMembership
  ] ; 
  rdfs:comment "A container for all the information about a single person." .

lisp:user_id rdf:type rdf:Property ;
  rdfs:domain lisp:LISPerson ;
  rdfs:range xsd:normalizedString ;
  rdfs:comment "A unique identifier for the person." .

lisp:sourcedId rdf:type rdf:Property ;
  rdfs:domain lisp:LISPerson ;
  rdfs:range xsd:normalizedString ;
  rdfs:comment "A unique identifier for the person as provisioned by an external system such as an SIS." .

lisp:email rdf:type rdf:Property ;
  rdfs:domain lisp:LISPerson ;
  rdfs:range xsd:string ;
  rdfs:comment "The primary email address for the person." .

lisp:resultSourcedId rdf:type rdf:Property ;
  rdfs:domain lisp:LISPerson ;
  rdfs:range xsd:string ;
  rdfs:comment "The person's LIS Result Identifier (if any) associated with a launch from the organization.  This will normally only have a value if the organization represents a resource link, though could also reflect a course-level launch." .

