<?xml version="1.0"?>


<!DOCTYPE rdf:RDF [
    <!ENTITY owl "http://www.w3.org/2002/07/owl#" >
    <!ENTITY xsd "http://www.w3.org/2001/XMLSchema#" >
    <!ENTITY xml "http://www.w3.org/XML/1998/namespace" >
    <!ENTITY rdfs "http://www.w3.org/2000/01/rdf-schema#" >
    <!ENTITY ci "http://purl.imsglobal.org/vocab/lti/v1/ci#" >
    <!ENTITY lti-type "http://purl.imsglobal.org/xsd/lti/v2/ltid#" >
    <!ENTITY rdf "http://www.w3.org/1999/02/22-rdf-syntax-ns#" >
    <!ENTITY lti "http://purl.imsglobal.org/vocab/lti/v2/lti#" >
    <!ENTITY bind "http://purl.org/semantictools/v1/vocab/bind#" >
    <!ENTITY liso "http://purl.imsglobal.org/vocab/lis/v2/outcomes#" >
]>


<rdf:RDF xmlns="http://www.semanticweb.org/owl/owlapi/turtle#"
     xml:base="http://www.semanticweb.org/owl/owlapi/turtle"
     xmlns:rdfs="http://www.w3.org/2000/01/rdf-schema#"
     xmlns:lti-type="http://purl.imsglobal.org/xsd/lti/v2/ltid#"
     xmlns:lti="http://purl.imsglobal.org/vocab/lti/v2/lti#"
     xmlns:ci="http://purl.imsglobal.org/vocab/lti/v1/ci#"
     xmlns:owl="http://www.w3.org/2002/07/owl#"
     xmlns:xsd="http://www.w3.org/2001/XMLSchema#"
     xmlns:rdf="http://www.w3.org/1999/02/22-rdf-syntax-ns#"
     xmlns:xml="http://www.w3.org/XML/1998/namespace"
     xmlns:liso="http://purl.imsglobal.org/vocab/lis/v2/outcomes#"
     xmlns:bind="http://purl.org/semantictools/v1/vocab/bind#">
    <owl:Ontology rdf:about="http://purl.imsglobal.org/vocab/lti/v2/lti#">
        <rdfs:label>LTI Core</rdfs:label>
        <bind:suggestedPrefix>lti</bind:suggestedPrefix>
    </owl:Ontology>
    


    <!-- 
    ///////////////////////////////////////////////////////////////////////////////////////
    //
    // Object Properties
    //
    ///////////////////////////////////////////////////////////////////////////////////////
     -->

    


    <!-- http://purl.imsglobal.org/vocab/lis/v2/outcomes#lineItemOf -->

    <owl:ObjectProperty rdf:about="&liso;lineItemOf"/>
    


    <!-- http://purl.imsglobal.org/vocab/lti/v2/lti#action -->

    <owl:ObjectProperty rdf:about="&lti;action">
        <rdfs:comment>Specifies an HTTP method (POST, GET, PUT, etc.) which the integration partner intends to use.   A RestServiceProfile may include more than one action.  However, the set of actions declared in a RestServiceProfile must be a subset of actions declared in the RestService referenced by the &lt;code&gt;service&lt;/code&gt; property.</rdfs:comment>
        <rdfs:range rdf:resource="&lti;HttpMethod"/>
        <rdfs:domain>
            <owl:Class>
                <owl:unionOf rdf:parseType="Collection">
                    <rdf:Description rdf:about="&lti;RestService"/>
                    <rdf:Description rdf:about="&lti;RestServiceProfile"/>
                </owl:unionOf>
            </owl:Class>
        </rdfs:domain>
    </owl:ObjectProperty>
    


    <!-- http://purl.imsglobal.org/vocab/lti/v2/lti#applies_to -->

    <owl:ObjectProperty rdf:about="&lti;applies_to">
        <rdfs:comment>The class of resources selected by this BaseUrlSelector.</rdfs:comment>
        <rdfs:domain rdf:resource="&lti;BaseUrlSelector"/>
        <rdfs:range rdf:resource="&owl;Class"/>
    </owl:ObjectProperty>
    


    <!-- http://purl.imsglobal.org/vocab/lti/v2/lti#base_url_choice -->

    <owl:ObjectProperty rdf:about="&lti;base_url_choice">
        <rdfs:range rdf:resource="&lti;BaseUrlChoice"/>
        <rdfs:domain rdf:resource="&lti;ToolProfile"/>
    </owl:ObjectProperty>
    


    <!-- http://purl.imsglobal.org/vocab/lti/v2/lti#capability_offered -->

    <owl:ObjectProperty rdf:about="&lti;capability_offered">
        <rdfs:comment>A capability offered by the Tool Consumer to its integration partners.</rdfs:comment>
        <rdfs:range rdf:resource="&lti;Capability"/>
        <rdfs:domain rdf:resource="&lti;ToolConsumerProfile"/>
    </owl:ObjectProperty>
    


    <!-- http://purl.imsglobal.org/vocab/lti/v2/lti#code -->

    <owl:ObjectProperty rdf:about="&lti;code">
        <rdf:type rdf:resource="&owl;FunctionalProperty"/>
        <rdfs:comment>A unique identifier for the resource.</rdfs:comment>
        <rdfs:domain rdf:resource="&lti;HasCode"/>
        <rdfs:range rdf:resource="&lti-type;Token.Type"/>
    </owl:ObjectProperty>
    


    <!-- http://purl.imsglobal.org/vocab/lti/v2/lti#contact -->

    <owl:ObjectProperty rdf:about="&lti;contact">
        <rdf:type rdf:resource="&owl;FunctionalProperty"/>
        <rdfs:comment>Contact information for this Vendor.</rdfs:comment>
        <rdfs:range rdf:resource="&lti;Contact"/>
        <rdfs:domain rdf:resource="&lti;Vendor"/>
    </owl:ObjectProperty>
    


    <!-- http://purl.imsglobal.org/vocab/lti/v2/lti#context -->

    <owl:ObjectProperty rdf:about="&lti;context">
        <rdf:type rdf:resource="&owl;FunctionalProperty"/>
        <rdfs:comment>The learning Context associated with this &lt;code&gt;ToolProxyBinding&lt;/code&gt;.</rdfs:comment>
        <rdfs:range rdf:resource="&lti;Context"/>
        <rdfs:domain rdf:resource="&lti;ToolProxyBinding"/>
    </owl:ObjectProperty>
    


    <!-- http://purl.imsglobal.org/vocab/lti/v2/lti#context_id -->

    <owl:ObjectProperty rdf:about="&lti;context_id">
        <rdf:type rdf:resource="&owl;FunctionalProperty"/>
        <rdfs:comment>A unique string provided by the tool consumer to identify the context (as passed in the context_id launch parameter).</rdfs:comment>
        <rdfs:domain rdf:resource="&lti;Context"/>
        <rdfs:range rdf:resource="&xsd;normalizedString"/>
    </owl:ObjectProperty>
    


    <!-- http://purl.imsglobal.org/vocab/lti/v2/lti#custom -->

    <owl:ObjectProperty rdf:about="&lti;custom">
        <rdf:type rdf:resource="&owl;FunctionalProperty"/>
        <rdfs:comment>A collection of custom properties defined by the Tool Provider and stored in this ToolSettingsContainer.</rdfs:comment>
        <rdfs:range rdf:resource="&lti;PropertyMap"/>
        <rdfs:domain rdf:resource="&lti;ToolSettingsContainer"/>
    </owl:ObjectProperty>
    


    <!-- http://purl.imsglobal.org/vocab/lti/v2/lti#default_location -->

    <owl:ObjectProperty rdf:about="&lti;default_location">
        <rdf:type rdf:resource="&owl;FunctionalProperty"/>
        <rdfs:comment>Specifies the default path to an icon.  The absolute URL is formed by appending this path to the appropriate base URL for icons.</rdfs:comment>
        <rdfs:range rdf:resource="&lti;IconEndpoint"/>
        <rdfs:domain rdf:resource="&lti;IconInfo"/>
    </owl:ObjectProperty>
    


    <!-- http://purl.imsglobal.org/vocab/lti/v2/lti#default_value -->

    <owl:ObjectProperty rdf:about="&lti;default_value">
        <rdf:type rdf:resource="&owl;FunctionalProperty"/>
        <rdfs:comment>The default value for the display name.  This value is used if (1) the key attribute is undefined, (2) the localization capability is not enabled, or (3) a value for the specified key is not found in the locale-specific resource bundle.</rdfs:comment>
        <rdfs:domain>
            <owl:Class>
                <owl:unionOf rdf:parseType="Collection">
                    <rdf:Description rdf:about="&lti;LocalizedName"/>
                    <rdf:Description rdf:about="&lti;LocalizedText"/>
                    <rdf:Description rdf:about="&lti;ShortLocalizedName"/>
                </owl:unionOf>
            </owl:Class>
        </rdfs:domain>
        <rdfs:range>
            <owl:Class>
                <owl:unionOf rdf:parseType="Collection">
                    <rdf:Description rdf:about="&lti-type;LongName.Type"/>
                    <rdf:Description rdf:about="&lti-type;ShortName.Type"/>
                    <rdf:Description rdf:about="&lti-type;Text.Type"/>
                </owl:unionOf>
            </owl:Class>
        </rdfs:range>
    </owl:ObjectProperty>
    


    <!-- http://purl.imsglobal.org/vocab/lti/v2/lti#description -->

    <owl:ObjectProperty rdf:about="&lti;description">
        <rdf:type rdf:resource="&owl;FunctionalProperty"/>
        <rdfs:comment>A description of the service provider, suitable for display to end-users.</rdfs:comment>
        <rdfs:range rdf:resource="&lti;LocalizedText"/>
        <rdfs:domain>
            <owl:Class>
                <owl:unionOf rdf:parseType="Collection">
                    <rdf:Description rdf:about="&lti;ProductInfo"/>
                    <rdf:Description rdf:about="&lti;ResourceHandler"/>
                    <rdf:Description rdf:about="&lti;ServiceOwner"/>
                    <rdf:Description rdf:about="&lti;ServiceProvider"/>
                    <rdf:Description rdf:about="&lti;Vendor"/>
                </owl:unionOf>
            </owl:Class>
        </rdfs:domain>
    </owl:ObjectProperty>
    


    <!-- http://purl.imsglobal.org/vocab/lti/v2/lti#email -->

    <owl:ObjectProperty rdf:about="&lti;email">
        <rdf:type rdf:resource="&owl;FunctionalProperty"/>
        <rdfs:comment>The email of the primary contact for the associated object.</rdfs:comment>
        <rdfs:domain rdf:resource="&lti;Contact"/>
        <rdfs:range rdf:resource="&xsd;normalizedString"/>
    </owl:ObjectProperty>
    


    <!-- http://purl.imsglobal.org/vocab/lti/v2/lti#enabled_capability -->

    <owl:ObjectProperty rdf:about="&lti;enabled_capability">
        <rdfs:comment>A capability that is enabled for messages handled by this MessageHandler.</rdfs:comment>
        <rdfs:range rdf:resource="&lti;Capability"/>
        <rdfs:domain>
            <owl:Class>
                <owl:unionOf rdf:parseType="Collection">
                    <rdf:Description rdf:about="&lti;MessageHandler"/>
                    <rdf:Description rdf:about="&lti;ToolProxy"/>
                </owl:unionOf>
            </owl:Class>
        </rdfs:domain>
    </owl:ObjectProperty>
    


    <!-- http://purl.imsglobal.org/vocab/lti/v2/lti#end_user_service -->

    <owl:ObjectProperty rdf:about="&lti;end_user_service">
        <rdfs:comment>The profile for a Tool Consumer service that may be invoked by the Tool when acting as an agent for some end user.  </rdfs:comment>
        <rdfs:domain rdf:resource="&lti;SecurityContract"/>
        <rdfs:range rdf:resource="&lti;ServiceProfile"/>
    </owl:ObjectProperty>
    


    <!-- http://purl.imsglobal.org/vocab/lti/v2/lti#fixed -->

    <owl:ObjectProperty rdf:about="&lti;fixed">
        <rdf:type rdf:resource="&owl;FunctionalProperty"/>
        <rdfs:comment>Denotes that the value of the parameter is fixed at the time of definition within the product profile.  This value must be passed in each message of the associated message type.</rdfs:comment>
        <rdfs:domain rdf:resource="&lti;Parameter"/>
        <rdfs:range rdf:resource="&lti-type;DataValue.Type"/>
    </owl:ObjectProperty>
    


    <!-- http://purl.imsglobal.org/vocab/lti/v2/lti#format -->

    <owl:ObjectProperty rdf:about="&lti;format">
        <rdfs:comment>The content type (also known as media type) of resources accessed via the endpoint defined by this RestService descriptor.   The endpoint of a REST service may support more than one content type if content negotiation is enabled as described in the &lt;a href=&quot;http://www.w3.org/Protocols/rfc2616/rfc2616-sec12.html&quot;&gt;HTTP 1.1&lt;/a&gt; specification.</rdfs:comment>
        <rdfs:domain rdf:resource="&lti;RestService"/>
        <rdfs:range rdf:resource="&xsd;normalizedString"/>
    </owl:ObjectProperty>
    


    <!-- http://purl.imsglobal.org/vocab/lti/v2/lti#guid -->

    <owl:ObjectProperty rdf:about="&lti;guid">
        <rdf:type rdf:resource="&owl;FunctionalProperty"/>
        <rdfs:comment>A globally unique identifier for the service provider.  As a best practice, this value should match an Internet domain name assigned by ICANN, but any globally unique identifier is acceptable.  </rdfs:comment>
        <rdfs:range rdf:resource="&lti-type;GUID.Type"/>
        <rdfs:domain>
            <owl:Class>
                <owl:unionOf rdf:parseType="Collection">
                    <rdf:Description rdf:about="&lti;ProductInstance"/>
                    <rdf:Description rdf:about="&lti;ServiceProvider"/>
                    <rdf:Description rdf:about="&lti;ToolConsumerProfile"/>
                </owl:unionOf>
            </owl:Class>
        </rdfs:domain>
    </owl:ObjectProperty>
    


    <!-- http://purl.imsglobal.org/vocab/lti/v2/lti#http_method -->

    <owl:ObjectProperty rdf:about="&lti;http_method">
        <rdfs:comment>Specifies an HTTP method (POST, GET, PUT, etc.) for the type of messages represented by this MessageType.</rdfs:comment>
        <rdfs:range rdf:resource="&lti;HttpMethod"/>
        <rdfs:domain rdf:resource="&lti;MessageType"/>
    </owl:ObjectProperty>
    


    <!-- http://purl.imsglobal.org/vocab/lti/v2/lti#icon_info -->

    <owl:ObjectProperty rdf:about="&lti;icon_info">
        <rdfs:comment>Provides information about a graphical icon that represents the resource described by this ResourceHandler.</rdfs:comment>
        <rdfs:range rdf:resource="&lti;IconInfo"/>
        <rdfs:domain rdf:resource="&lti;ResourceHandler"/>
    </owl:ObjectProperty>
    


    <!-- http://purl.imsglobal.org/vocab/lti/v2/lti#icon_style -->

    <owl:ObjectProperty rdf:about="&lti;icon_style">
        <rdfs:comment>The style of the icon referenced by this IconInfo.</rdfs:comment>
        <rdfs:domain rdf:resource="&lti;IconInfo"/>
        <rdfs:range rdf:resource="&lti;IconStyle"/>
    </owl:ObjectProperty>
    


    <!-- http://purl.imsglobal.org/vocab/lti/v2/lti#instance -->

    <owl:ObjectProperty rdf:about="&lti;instance">
        <rdfs:comment>A deployed instance of a particular version of a product (Tool or Tool Consumer).</rdfs:comment>
        <rdfs:domain rdf:resource="&lti;ProductInfo"/>
        <rdfs:range rdf:resource="&lti;ProductInstance"/>
    </owl:ObjectProperty>
    


    <!-- http://purl.imsglobal.org/vocab/lti/v2/lti#key -->

    <owl:ObjectProperty rdf:about="&lti;key">
        <rdf:type rdf:resource="&owl;FunctionalProperty"/>
        <rdfs:comment>If localization is supported then the &apos;key&apos; attribute identifies a property in the resource bundle provided in response to the get-bundle-request message. The value of that property is the locale-specific path to the icon.</rdfs:comment>
        <rdfs:range rdf:resource="&lti-type;Name.Type"/>
        <rdfs:domain>
            <owl:Class>
                <owl:unionOf rdf:parseType="Collection">
                    <rdf:Description rdf:about="&lti;IconInfo"/>
                    <rdf:Description rdf:about="&lti;LocalizedName"/>
                    <rdf:Description rdf:about="&lti;LocalizedText"/>
                    <rdf:Description rdf:about="&lti;ShortLocalizedName"/>
                </owl:unionOf>
            </owl:Class>
        </rdfs:domain>
    </owl:ObjectProperty>
    


    <!-- http://purl.imsglobal.org/vocab/lti/v2/lti#lineItem -->

    <owl:ObjectProperty rdf:about="&lti;lineItem">
        <rdfs:comment>A LineItem that records results for some learning activity within this context.</rdfs:comment>
        <rdfs:range rdf:resource="&liso;LineItem"/>
        <owl:inverseOf rdf:resource="&liso;lineItemOf"/>
        <rdfs:domain rdf:resource="&lti;Context"/>
    </owl:ObjectProperty>
    


    <!-- http://purl.imsglobal.org/vocab/lti/v2/lti#lineItems -->

    <owl:ObjectProperty rdf:about="&lti;lineItems">
        <rdf:type rdf:resource="&owl;FunctionalProperty"/>
        <rdfs:range rdf:resource="&liso;LineItemContainer"/>
        <rdfs:domain rdf:resource="&lti;Context"/>
    </owl:ObjectProperty>
    


    <!-- http://purl.imsglobal.org/vocab/lti/v2/lti#linkLineItem -->

    <owl:ObjectProperty rdf:about="&lti;linkLineItem">
        <rdf:type rdf:resource="&owl;FunctionalProperty"/>
        <rdfs:range rdf:resource="&liso;LineItem"/>
        <rdfs:domain rdf:resource="&lti;AssignmentLink"/>
    </owl:ObjectProperty>
    


    <!-- http://purl.imsglobal.org/vocab/lti/v2/lti#lti_version -->

    <owl:ObjectProperty rdf:about="&lti;lti_version">
        <rdf:type rdf:resource="&owl;FunctionalProperty"/>
        <rdfs:comment>The identifier for an LTI version that the version supports.  A given product (Tool or Tool Consumer) may support multiple versions, but only one version is selected for use in the integration contract.</rdfs:comment>
        <rdfs:domain>
            <owl:Class>
                <owl:unionOf rdf:parseType="Collection">
                    <rdf:Description rdf:about="&lti;ProductProfile"/>
                    <rdf:Description rdf:about="&lti;ToolProxy"/>
                </owl:unionOf>
            </owl:Class>
        </rdfs:domain>
        <rdfs:range>
            <owl:Class>
                <owl:unionOf rdf:parseType="Collection">
                    <rdf:Description rdf:about="&xsd;normalizedString"/>
                    <rdf:Description rdf:about="&xsd;token"/>
                </owl:unionOf>
            </owl:Class>
        </rdfs:range>
    </owl:ObjectProperty>
    


    <!-- http://purl.imsglobal.org/vocab/lti/v2/lti#message -->

    <owl:ObjectProperty rdf:about="&lti;message">
        <rdfs:range rdf:resource="&lti;MessageHandler"/>
        <rdfs:domain>
            <owl:Class>
                <owl:unionOf rdf:parseType="Collection">
                    <rdf:Description rdf:about="&lti;ResourceHandler"/>
                    <rdf:Description rdf:about="&lti;ToolProfile"/>
                </owl:unionOf>
            </owl:Class>
        </rdfs:domain>
    </owl:ObjectProperty>
    


    <!-- http://purl.imsglobal.org/vocab/lti/v2/lti#message_class -->

    <owl:ObjectProperty rdf:about="&lti;message_class">
        <rdf:type rdf:resource="&owl;FunctionalProperty"/>
        <rdfs:comment>This attribute identifies the formal Class definition the type of message that can be delivered to a given MessageHandler.</rdfs:comment>
        <rdfs:domain rdf:resource="&lti;MessageType"/>
        <rdfs:range rdf:resource="&owl;Class"/>
    </owl:ObjectProperty>
    


    <!-- http://purl.imsglobal.org/vocab/lti/v2/lti#message_type -->

    <owl:ObjectProperty rdf:about="&lti;message_type">
        <rdf:type rdf:resource="&owl;FunctionalProperty"/>
        <rdfs:comment>The type of message that can be submitted to the Message Handler.</rdfs:comment>
        <rdfs:domain rdf:resource="&lti;MessageHandler"/>
        <rdfs:range rdf:resource="&lti;MessageType"/>
    </owl:ObjectProperty>
    


    <!-- http://purl.imsglobal.org/vocab/lti/v2/lti#parameter -->

    <owl:ObjectProperty rdf:about="&lti;parameter">
        <rdfs:comment>Specifies a custom parameter that is expected by the MessageHandler.</rdfs:comment>
        <rdfs:domain rdf:resource="&lti;MessageHandler"/>
        <rdfs:range rdf:resource="&lti;Parameter"/>
    </owl:ObjectProperty>
    


    <!-- http://purl.imsglobal.org/vocab/lti/v2/lti#product -->

    <owl:ObjectProperty rdf:about="&lti;product">
        <rdfs:comment>&lt;p&gt;A group of related products offered by the Vendor.  All of the products within a given product family are different &lt;em&gt;versions&lt;/em&gt; of the same product. &lt;/p&gt;
&lt;p&gt;A vendor may have multiple product families.  For example, the same vendor might offer a discussion forum tool and also a white board tool.  Each of these tools corresponds to a different product family.&lt;/p&gt;</rdfs:comment>
        <rdfs:range rdf:resource="&lti;ProductFamily"/>
        <rdfs:domain rdf:resource="&lti;Vendor"/>
    </owl:ObjectProperty>
    


    <!-- http://purl.imsglobal.org/vocab/lti/v2/lti#product_family -->

    <owl:ObjectProperty rdf:about="&lti;product_family">
        <rdf:type rdf:resource="&owl;FunctionalProperty"/>
        <rdfs:comment>An inverse attribute that references the ProductFamily within which this ProductInfo is defined.</rdfs:comment>
        <rdfs:range rdf:resource="&lti;ProductFamily"/>
        <rdfs:domain rdf:resource="&lti;ProductInfo"/>
    </owl:ObjectProperty>
    


    <!-- http://purl.imsglobal.org/vocab/lti/v2/lti#product_info -->

    <owl:ObjectProperty rdf:about="&lti;product_info">
        <rdf:type rdf:resource="&owl;FunctionalProperty"/>
        <rdfs:comment>This is metadata about the product described in the profile.</rdfs:comment>
        <rdfs:range rdf:resource="&lti;ProductInfo"/>
        <rdfs:domain rdf:resource="&lti;ProductInstance"/>
        <owl:inverseOf rdf:resource="&lti;instance"/>
    </owl:ObjectProperty>
    


    <!-- http://purl.imsglobal.org/vocab/lti/v2/lti#product_instance -->

    <owl:ObjectProperty rdf:about="&lti;product_instance">
        <rdf:type rdf:resource="&owl;FunctionalProperty"/>
        <rdfs:comment>An inverse attribute which references the ProductInstance within which this ProductProfile is defined.</rdfs:comment>
        <rdfs:range rdf:resource="&lti;ProductInstance"/>
        <rdfs:domain rdf:resource="&lti;ProductProfile"/>
        <owl:inverseOf rdf:resource="&lti;profile"/>
    </owl:ObjectProperty>
    


    <!-- http://purl.imsglobal.org/vocab/lti/v2/lti#product_name -->

    <owl:ObjectProperty rdf:about="&lti;product_name">
        <rdf:type rdf:resource="&owl;FunctionalProperty"/>
        <rdfs:comment>A name for the product, suitable for display to end users.</rdfs:comment>
        <rdfs:range rdf:resource="&lti;LocalizedName"/>
        <rdfs:domain rdf:resource="&lti;ProductInfo"/>
    </owl:ObjectProperty>
    


    <!-- http://purl.imsglobal.org/vocab/lti/v2/lti#profile -->

    <owl:ObjectProperty rdf:about="&lti;profile">
        <rdfs:comment>A resource that presents a view of this ProductInstance to one or more integration partners.</rdfs:comment>
        <rdfs:domain rdf:resource="&lti;ProductInstance"/>
        <rdfs:range rdf:resource="&lti;ProductProfile"/>
    </owl:ObjectProperty>
    


    <!-- http://purl.imsglobal.org/vocab/lti/v2/lti#resource_handler -->

    <owl:ObjectProperty rdf:about="&lti;resource_handler">
        <rdfs:range rdf:resource="&lti;ResourceHandler"/>
        <rdfs:domain rdf:resource="&lti;ToolProfile"/>
    </owl:ObjectProperty>
    


    <!-- http://purl.imsglobal.org/vocab/lti/v2/lti#resource_link_id -->

    <owl:ObjectProperty rdf:about="&lti;resource_link_id">
        <rdf:type rdf:resource="&owl;FunctionalProperty"/>
        <rdfs:comment>A globally unique identifier for this LTI link.</rdfs:comment>
        <rdfs:domain rdf:resource="&lti;LtiLink"/>
        <rdfs:range rdf:resource="&lti-type;GUID.Type"/>
    </owl:ObjectProperty>
    


    <!-- http://purl.imsglobal.org/vocab/lti/v2/lti#resource_name -->

    <owl:ObjectProperty rdf:about="&lti;resource_name">
        <rdf:type rdf:resource="&owl;FunctionalProperty"/>
        <rdfs:comment>The name of the resource handler suitable for display in the TC user interface.</rdfs:comment>
        <rdfs:range rdf:resource="&lti;LocalizedName"/>
        <rdfs:domain rdf:resource="&lti;ResourceHandler"/>
    </owl:ObjectProperty>
    


    <!-- http://purl.imsglobal.org/vocab/lti/v2/lti#resource_type -->

    <owl:ObjectProperty rdf:about="&lti;resource_type">
        <rdf:type rdf:resource="&owl;FunctionalProperty"/>
        <rdfs:comment>Identifies the type of resource associated with this ResourceHandler.  Resource types are identified by a code that is unique within a given ProductFamily.</rdfs:comment>
        <rdfs:domain rdf:resource="&lti;ResourceHandler"/>
        <rdfs:range rdf:resource="&lti;ResourceType"/>
    </owl:ObjectProperty>
    


    <!-- http://purl.imsglobal.org/vocab/lti/v2/lti#resource_type_owner -->

    <owl:ObjectProperty rdf:about="&lti;resource_type_owner">
        <rdf:type rdf:resource="&owl;FunctionalProperty"/>
        <rdfs:range rdf:resource="&lti;ProductFamily"/>
        <rdfs:domain rdf:resource="&lti;ResourceType"/>
    </owl:ObjectProperty>
    


    <!-- http://purl.imsglobal.org/vocab/lti/v2/lti#security_contract -->

    <owl:ObjectProperty rdf:about="&lti;security_contract">
        <rdf:type rdf:resource="&owl;FunctionalProperty"/>
        <rdfs:comment>The security aspect of an integration contract between two parties.</rdfs:comment>
        <rdfs:range rdf:resource="&lti;SecurityContract"/>
        <rdfs:domain rdf:resource="&lti;ToolProxy"/>
    </owl:ObjectProperty>
    


    <!-- http://purl.imsglobal.org/vocab/lti/v2/lti#selector -->

    <owl:ObjectProperty rdf:about="&lti;selector">
        <rdf:type rdf:resource="&owl;FunctionalProperty"/>
        <rdfs:comment>A resource that specifies the objects to which this BaseUrlChoice applies. </rdfs:comment>
        <rdfs:domain rdf:resource="&lti;BaseUrlChoice"/>
        <rdfs:range rdf:resource="&lti;BaseUrlSelector"/>
    </owl:ObjectProperty>
    


    <!-- http://purl.imsglobal.org/vocab/lti/v2/lti#service -->

    <owl:ObjectProperty rdf:about="&lti;service">
        <rdf:type rdf:resource="&owl;FunctionalProperty"/>
        <rdfs:comment>The descriptor for the service that is being profiled.</rdfs:comment>
        <rdfs:range rdf:resource="&lti;ServiceDescriptor"/>
        <rdfs:domain rdf:resource="&lti;ServiceProfile"/>
    </owl:ObjectProperty>
    


    <!-- http://purl.imsglobal.org/vocab/lti/v2/lti#service_offered -->

    <owl:ObjectProperty rdf:about="&lti;service_offered">
        <rdfs:comment>The descriptor for a service offered by the product (Tool or Tool Consumer).</rdfs:comment>
        <rdfs:domain rdf:resource="&lti;ProductProfile"/>
        <rdfs:range rdf:resource="&lti;ServiceDescriptor"/>
    </owl:ObjectProperty>
    


    <!-- http://purl.imsglobal.org/vocab/lti/v2/lti#service_owner -->

    <owl:ObjectProperty rdf:about="&lti;service_owner">
        <rdf:type rdf:resource="&owl;FunctionalProperty"/>
        <rdfs:comment>The entity that owns the services provided by this product instance.</rdfs:comment>
        <rdfs:domain rdf:resource="&lti;ProductInstance"/>
        <rdfs:range rdf:resource="&lti;ServiceOwner"/>
    </owl:ObjectProperty>
    


    <!-- http://purl.imsglobal.org/vocab/lti/v2/lti#service_owner_name -->

    <owl:ObjectProperty rdf:about="&lti;service_owner_name">
        <rdf:type rdf:resource="&owl;FunctionalProperty"/>
        <rdfs:range rdf:resource="&lti;LocalizedName"/>
        <rdfs:domain rdf:resource="&lti;ServiceOwner"/>
    </owl:ObjectProperty>
    


    <!-- http://purl.imsglobal.org/vocab/lti/v2/lti#service_provider -->

    <owl:ObjectProperty rdf:about="&lti;service_provider">
        <rdf:type rdf:resource="&owl;FunctionalProperty"/>
        <rdfs:comment>This is the service provider that hosts the deployed product.</rdfs:comment>
        <rdfs:domain rdf:resource="&lti;ProductInstance"/>
        <rdfs:range rdf:resource="&lti;ServiceProvider"/>
    </owl:ObjectProperty>
    


    <!-- http://purl.imsglobal.org/vocab/lti/v2/lti#service_provider_name -->

    <owl:ObjectProperty rdf:about="&lti;service_provider_name">
        <rdf:type rdf:resource="&owl;FunctionalProperty"/>
        <rdfs:comment>The name of the service provider, suitable for display to end users.</rdfs:comment>
        <rdfs:range rdf:resource="&lti;LocalizedName"/>
        <rdfs:domain rdf:resource="&lti;ServiceProvider"/>
    </owl:ObjectProperty>
    


    <!-- http://purl.imsglobal.org/vocab/lti/v2/lti#support -->

    <owl:ObjectProperty rdf:about="&lti;support">
        <rdf:type rdf:resource="&owl;FunctionalProperty"/>
        <rdfs:comment>Contact information for support from a service provider.</rdfs:comment>
        <rdfs:range rdf:resource="&lti;Contact"/>
        <rdfs:domain>
            <owl:Class>
                <owl:unionOf rdf:parseType="Collection">
                    <rdf:Description rdf:about="&lti;ProductInstance"/>
                    <rdf:Description rdf:about="&lti;ServiceProvider"/>
                </owl:unionOf>
            </owl:Class>
        </rdfs:domain>
    </owl:ObjectProperty>
    


    <!-- http://purl.imsglobal.org/vocab/lti/v2/lti#technical_description -->

    <owl:ObjectProperty rdf:about="&lti;technical_description">
        <rdf:type rdf:resource="&owl;FunctionalProperty"/>
        <rdfs:comment>This is a human readable description of the technical aspects of this product that might be of interest to developers who wish to integrate with this product via LTI.</rdfs:comment>
        <rdfs:range rdf:resource="&lti;LocalizedText"/>
        <rdfs:domain rdf:resource="&lti;ProductInfo"/>
    </owl:ObjectProperty>
    


    <!-- http://purl.imsglobal.org/vocab/lti/v2/lti#tool_consumer_profile -->

    <owl:ObjectProperty rdf:about="&lti;tool_consumer_profile">
        <rdf:type rdf:resource="&owl;FunctionalProperty"/>
        <rdfs:comment>The profile of the Tool Consumer that is participating in the integration governed by this ToolProxy.</rdfs:comment>
        <rdfs:range rdf:resource="&lti;ToolConsumerProfile"/>
        <rdfs:domain rdf:resource="&lti;ToolProxy"/>
    </owl:ObjectProperty>
    


    <!-- http://purl.imsglobal.org/vocab/lti/v2/lti#tool_profile -->

    <owl:ObjectProperty rdf:about="&lti;tool_profile">
        <rdf:type rdf:resource="&owl;FunctionalProperty"/>
        <rdfs:comment>The profile of the Tool that is participating in the integration governed by this ToolProxy.</rdfs:comment>
        <rdfs:range rdf:resource="&lti;ToolProfile"/>
        <rdfs:domain rdf:resource="&lti;ToolProxy"/>
    </owl:ObjectProperty>
    


    <!-- http://purl.imsglobal.org/vocab/lti/v2/lti#tool_proxy_guid -->

    <owl:ObjectProperty rdf:about="&lti;tool_proxy_guid">
        <rdf:type rdf:resource="&owl;FunctionalProperty"/>
        <rdfs:comment>The globally unique identifier for the ToolProxy (a.k.a. integration contract).</rdfs:comment>
        <rdfs:domain rdf:resource="&lti;ToolProxy"/>
        <rdfs:range rdf:resource="&lti-type;GUID.Type"/>
    </owl:ObjectProperty>
    


    <!-- http://purl.imsglobal.org/vocab/lti/v2/lti#tool_service -->

    <owl:ObjectProperty rdf:about="&lti;tool_service">
        <rdfs:comment>The profile for a Tool Consumer service that may be invoked by the Tool acting on its own (as opposed to acting as an agent for some end user).  </rdfs:comment>
        <rdfs:domain rdf:resource="&lti;SecurityContract"/>
        <rdfs:range rdf:resource="&lti;ServiceProfile"/>
    </owl:ObjectProperty>
    


    <!-- http://purl.imsglobal.org/vocab/lti/v2/lti#variable -->

    <owl:ObjectProperty rdf:about="&lti;variable">
        <rdf:type rdf:resource="&owl;FunctionalProperty"/>
        <rdfs:comment>Denotes that the parameter has a variable value that is automatically substituted at run-time.  The value of this attribute is the name for a variable whose value will be added to the message at run-time. </rdfs:comment>
        <rdfs:domain rdf:resource="&lti;Parameter"/>
        <rdfs:range rdf:resource="&lti-type;VariableName.Type"/>
    </owl:ObjectProperty>
    


    <!-- http://purl.imsglobal.org/vocab/lti/v2/lti#vendor -->

    <owl:ObjectProperty rdf:about="&lti;vendor">
        <rdf:type rdf:resource="&owl;FunctionalProperty"/>
        <rdfs:comment>The vendor that owns the ProductFamily.</rdfs:comment>
        <rdfs:domain rdf:resource="&lti;ProductFamily"/>
        <rdfs:range rdf:resource="&lti;Vendor"/>
        <owl:inverseOf rdf:resource="&lti;product"/>
    </owl:ObjectProperty>
    


    <!-- http://purl.imsglobal.org/vocab/lti/v2/lti#vendor_name -->

    <owl:ObjectProperty rdf:about="&lti;vendor_name">
        <rdf:type rdf:resource="&owl;FunctionalProperty"/>
        <rdfs:comment>Defines a human readable name for the Vendor.  The name should be suitable for display in management screens within the Tool Provider system.</rdfs:comment>
        <rdfs:range rdf:resource="&lti;LocalizedName"/>
        <rdfs:domain rdf:resource="&lti;Vendor"/>
    </owl:ObjectProperty>
    


    <!-- http://purl.imsglobal.org/vocab/lti/v2/lti#version -->

    <owl:ObjectProperty rdf:about="&lti;version">
        <rdfs:comment>Encapsulates information about one version of the product.</rdfs:comment>
        <rdfs:domain rdf:resource="&lti;ProductFamily"/>
        <rdfs:range rdf:resource="&lti;ProductInfo"/>
        <owl:inverseOf rdf:resource="&lti;product_family"/>
    </owl:ObjectProperty>
    


    <!-- 
    ///////////////////////////////////////////////////////////////////////////////////////
    //
    // Data properties
    //
    ///////////////////////////////////////////////////////////////////////////////////////
     -->

    


    <!-- http://purl.imsglobal.org/vocab/lti/v2/lti#absolute_path_allowed -->

    <owl:DatatypeProperty rdf:about="&lti;absolute_path_allowed">
        <rdf:type rdf:resource="&owl;FunctionalProperty"/>
        <rdfs:comment>Specifies whether the path for this message type is allowed to be specified using an absolute path.  A value of &quot;false&quot; means that the MessageHandler must declare a relative path.</rdfs:comment>
        <rdfs:domain rdf:resource="&lti;MessageType"/>
        <rdfs:range rdf:resource="&xsd;boolean"/>
    </owl:DatatypeProperty>
    


    <!-- http://purl.imsglobal.org/vocab/lti/v2/lti#custom_url -->

    <owl:DatatypeProperty rdf:about="&lti;custom_url">
        <rdf:type rdf:resource="&owl;FunctionalProperty"/>
        <rdfs:comment>The REST endpoint at which custom tool settings may be accessed for this ToolSettingsContainer.</rdfs:comment>
        <rdfs:domain rdf:resource="&lti;ToolSettingsContainer"/>
        <rdfs:range rdf:resource="&xsd;anyURI"/>
    </owl:DatatypeProperty>
    


    <!-- http://purl.imsglobal.org/vocab/lti/v2/lti#default_base_url -->

    <owl:DatatypeProperty rdf:about="&lti;default_base_url">
        <rdf:type rdf:resource="&owl;FunctionalProperty"/>
        <rdfs:comment>This is the base URL that should be used by default for all entities specified by the associated BaseUrlSelector.  The secure_base_url attribute may override this default Base URL.</rdfs:comment>
        <rdfs:domain rdf:resource="&lti;BaseUrlChoice"/>
        <rdfs:range rdf:resource="&xsd;anyURI"/>
    </owl:DatatypeProperty>
    


    <!-- http://purl.imsglobal.org/vocab/lti/v2/lti#endpoint -->

    <owl:DatatypeProperty rdf:about="&lti;endpoint">
        <rdf:type rdf:resource="&owl;FunctionalProperty"/>
        <rdfs:comment>A URI template that defines the REST endpoint for resources that may be accessed via the REST service.  The URI template should conform to the syntax in the proposed IETF standard [&lt;a href=&quot;http://www.ietf.org/id/draft-gregorio-uritemplate-08.txt&quot;&gt;draft-gregorio-uritemplate-08&lt;/a&gt;]. </rdfs:comment>
        <rdfs:domain rdf:resource="&lti;RestService"/>
        <rdfs:range rdf:resource="&xsd;anyURI"/>
    </owl:DatatypeProperty>
    


    <!-- http://purl.imsglobal.org/vocab/lti/v2/lti#name -->

    <owl:DatatypeProperty rdf:about="&lti;name">
        <rdf:type rdf:resource="&owl;FunctionalProperty"/>
        <rdfs:comment>The name of the parameter.</rdfs:comment>
        <rdfs:domain rdf:resource="&lti;Parameter"/>
        <rdfs:range rdf:resource="&xsd;Name"/>
    </owl:DatatypeProperty>
    


    <!-- http://purl.imsglobal.org/vocab/lti/v2/lti#path -->

    <owl:DatatypeProperty rdf:about="&lti;path">
        <rdf:type rdf:resource="&owl;FunctionalProperty"/>
        <rdfs:comment>This attribute specifies the path for an endpoint such as a MessageHandler or an Icon. Typically, this path is relative to one of the base URL values defined in a BaseUrlChoice.  
In the case of a MessageHandler, the path may be an absolute path if the associated message type explicitly declares that an absolute path is allowed.  </rdfs:comment>
        <rdfs:domain rdf:resource="&lti;Endpoint"/>
        <rdfs:range rdf:resource="&xsd;anyURI"/>
    </owl:DatatypeProperty>
    


    <!-- http://purl.imsglobal.org/vocab/lti/v2/lti#product_version -->

    <owl:DatatypeProperty rdf:about="&lti;product_version">
        <rdf:type rdf:resource="&owl;FunctionalProperty"/>
        <rdfs:comment>This is the version of the product. </rdfs:comment>
        <rdfs:domain rdf:resource="&lti;ProductInfo"/>
        <rdfs:range rdf:resource="&xsd;normalizedString"/>
    </owl:DatatypeProperty>
    


    <!-- http://purl.imsglobal.org/vocab/lti/v2/lti#secure_base_url -->

    <owl:DatatypeProperty rdf:about="&lti;secure_base_url">
        <rdf:type rdf:resource="&owl;FunctionalProperty"/>
        <rdfs:comment>This is the base URL that should be used whenever security is enabled.  If this base URL is not defined, then the default_base_url is used in all circumstances.</rdfs:comment>
        <rdfs:domain rdf:resource="&lti;BaseUrlChoice"/>
        <rdfs:range rdf:resource="&xsd;anyURI"/>
    </owl:DatatypeProperty>
    


    <!-- http://purl.imsglobal.org/vocab/lti/v2/lti#shared_secret -->

    <owl:DatatypeProperty rdf:about="&lti;shared_secret">
        <rdf:type rdf:resource="&owl;FunctionalProperty"/>
        <rdfs:comment>This is the shared secret used for communications between the Tool Consumer and the Tool Provider.  It is expected that the Tool Consumer present an interface to the administrative user for them to activate the Tool Proxy before this secret is ever used by the Tool Consumer. 
The shared secret may be updated when a tool is re-registered (see the reregisterTool operation of the ToolRegistrationService).  In addition, the TC and TP should provide interfaces which allow their respective administrators to change the shared secret through an out-of-band agreement.</rdfs:comment>
        <rdfs:domain rdf:resource="&lti;SecurityContract"/>
        <rdfs:range rdf:resource="&xsd;string"/>
    </owl:DatatypeProperty>
    


    <!-- http://purl.imsglobal.org/vocab/lti/v2/lti#sourcedId -->

    <owl:DatatypeProperty rdf:about="&lti;sourcedId">
        <rdf:type rdf:resource="&owl;FunctionalProperty"/>
        <rdfs:domain rdf:resource="&lti;Context"/>
        <rdfs:range rdf:resource="&xsd;normalizedString"/>
    </owl:DatatypeProperty>
    


    <!-- http://purl.imsglobal.org/vocab/lti/v2/lti#timestamp -->

    <owl:DatatypeProperty rdf:about="&lti;timestamp">
        <rdf:type rdf:resource="&owl;FunctionalProperty"/>
        <rdfs:comment>A timestamp for the ServiceProvider record. This value is useful for determining which record is most current.</rdfs:comment>
        <rdfs:range rdf:resource="&xsd;dateTime"/>
        <rdfs:domain>
            <owl:Class>
                <owl:unionOf rdf:parseType="Collection">
                    <rdf:Description rdf:about="&lti;ServiceOwner"/>
                    <rdf:Description rdf:about="&lti;ServiceProvider"/>
                    <rdf:Description rdf:about="&lti;Vendor"/>
                </owl:unionOf>
            </owl:Class>
        </rdfs:domain>
    </owl:DatatypeProperty>
    


    <!-- http://purl.imsglobal.org/vocab/lti/v2/lti#website -->

    <owl:DatatypeProperty rdf:about="&lti;website">
        <rdf:type rdf:resource="&owl;FunctionalProperty"/>
        <rdfs:comment>This is the URL of the vendor.</rdfs:comment>
        <rdfs:domain rdf:resource="&lti;Vendor"/>
        <rdfs:range rdf:resource="&xsd;anyURI"/>
    </owl:DatatypeProperty>
    


    <!-- 
    ///////////////////////////////////////////////////////////////////////////////////////
    //
    // Classes
    //
    ///////////////////////////////////////////////////////////////////////////////////////
     -->

    


    <!-- http://purl.imsglobal.org/vocab/lis/v2/outcomes#LineItem -->

    <owl:Class rdf:about="&liso;LineItem"/>
    


    <!-- http://purl.imsglobal.org/vocab/lis/v2/outcomes#LineItemContainer -->

    <owl:Class rdf:about="&liso;LineItemContainer"/>
    


    <!-- http://purl.imsglobal.org/vocab/lti/v1/ci#ContentItem -->

    <owl:Class rdf:about="&ci;ContentItem"/>
    


    <!-- http://purl.imsglobal.org/vocab/lti/v2/lti#AssignmentLink -->

    <owl:Class rdf:about="&lti;AssignmentLink">
        <rdfs:subClassOf rdf:resource="&lti;LtiLink"/>
    </owl:Class>
    


    <!-- http://purl.imsglobal.org/vocab/lti/v2/lti#BaseUrlChoice -->

    <owl:Class rdf:about="&lti;BaseUrlChoice">
        <rdfs:subClassOf>
            <owl:Restriction>
                <owl:onProperty rdf:resource="&lti;default_base_url"/>
                <owl:minCardinality rdf:datatype="&xsd;nonNegativeInteger">1</owl:minCardinality>
            </owl:Restriction>
        </rdfs:subClassOf>
        <rdfs:comment>Defines the base URL that is used for certain kinds of resources referenced in a ToolProfile.  The kinds of resources to which the base URL applies is specified by an associated BaseUrlSelector.  If the BaseUrlChoice does not have an associated selector, then it applies universally to all resources referenced in the Tool Profile. </rdfs:comment>
    </owl:Class>
    


    <!-- http://purl.imsglobal.org/vocab/lti/v2/lti#BaseUrlSelector -->

    <owl:Class rdf:about="&lti;BaseUrlSelector">
        <rdfs:subClassOf>
            <owl:Restriction>
                <owl:onProperty rdf:resource="&lti;applies_to"/>
                <owl:minCardinality rdf:datatype="&xsd;nonNegativeInteger">1</owl:minCardinality>
            </owl:Restriction>
        </rdfs:subClassOf>
        <rdfs:comment>This resource specifies the type of objects to which a set of base URLs apply. </rdfs:comment>
    </owl:Class>
    


    <!-- http://purl.imsglobal.org/vocab/lti/v2/lti#Capability -->

    <owl:Class rdf:about="&lti;Capability">
        <rdfs:comment>Represents a capability that may be declared by a Tool Consumer in its profile and enabled by a Tool when an integration contract is established.</rdfs:comment>
    </owl:Class>
    


    <!-- http://purl.imsglobal.org/vocab/lti/v2/lti#Contact -->

    <owl:Class rdf:about="&lti;Contact">
        <rdfs:subClassOf>
            <owl:Restriction>
                <owl:onProperty rdf:resource="&lti;email"/>
                <owl:minCardinality rdf:datatype="&xsd;nonNegativeInteger">1</owl:minCardinality>
            </owl:Restriction>
        </rdfs:subClassOf>
        <rdfs:comment>Contact information for the associated object.</rdfs:comment>
    </owl:Class>
    


    <!-- http://purl.imsglobal.org/vocab/lti/v2/lti#Context -->

    <owl:Class rdf:about="&lti;Context">
        <rdfs:subClassOf>
            <owl:Restriction>
                <owl:onProperty rdf:resource="&lti;context_id"/>
                <owl:minCardinality rdf:datatype="&xsd;nonNegativeInteger">1</owl:minCardinality>
            </owl:Restriction>
        </rdfs:subClassOf>
        <rdfs:comment>A learning context, such as a Course Section.</rdfs:comment>
    </owl:Class>
    


    <!-- http://purl.imsglobal.org/vocab/lti/v2/lti#DocumentTarget -->

    <owl:Class rdf:about="&lti;DocumentTarget"/>
    


    <!-- http://purl.imsglobal.org/vocab/lti/v2/lti#Endpoint -->

    <owl:Class rdf:about="&lti;Endpoint">
        <rdfs:subClassOf>
            <owl:Restriction>
                <owl:onProperty rdf:resource="&lti;path"/>
                <owl:minCardinality rdf:datatype="&xsd;nonNegativeInteger">1</owl:minCardinality>
            </owl:Restriction>
        </rdfs:subClassOf>
        <rdfs:comment>This is the abstract base class for objects that have an endpoint such as icons or message handlers. </rdfs:comment>
    </owl:Class>
    


    <!-- http://purl.imsglobal.org/vocab/lti/v2/lti#HasCode -->

    <owl:Class rdf:about="&lti;HasCode">
        <rdfs:subClassOf>
            <owl:Restriction>
                <owl:onProperty rdf:resource="&lti;code"/>
                <owl:minCardinality rdf:datatype="&xsd;nonNegativeInteger">1</owl:minCardinality>
            </owl:Restriction>
        </rdfs:subClassOf>
        <rdfs:comment>A resource that can be identified by a &lt;code&gt;code&lt;/code&gt; property.  The code property may be globally unique (as in the case of a Vendor resource) or locally unqiue (as in the case of a Product Family, where the code is locally unique within the scope of the parent Vendor resource).</rdfs:comment>
    </owl:Class>
    


    <!-- http://purl.imsglobal.org/vocab/lti/v2/lti#HttpMethod -->

    <owl:Class rdf:about="&lti;HttpMethod">
        <owl:equivalentClass>
            <owl:Class>
                <owl:oneOf rdf:parseType="Collection">
                    <rdf:Description rdf:about="&lti;GET"/>
                    <rdf:Description rdf:about="&lti;POST"/>
                </owl:oneOf>
            </owl:Class>
        </owl:equivalentClass>
        <rdfs:comment>Enumerates the HTTP methods that can be used when sending a message, as defined by IETF RFC 2616 .</rdfs:comment>
    </owl:Class>
    


    <!-- http://purl.imsglobal.org/vocab/lti/v2/lti#IconEndpoint -->

    <owl:Class rdf:about="&lti;IconEndpoint">
        <rdfs:subClassOf rdf:resource="&lti;Endpoint"/>
        <rdfs:comment>Defines the path for an Icon.  </rdfs:comment>
    </owl:Class>
    


    <!-- http://purl.imsglobal.org/vocab/lti/v2/lti#IconInfo -->

    <owl:Class rdf:about="&lti;IconInfo">
        <rdfs:comment>Contains information about a graphical icon that may be displayed in the Tool Consumer&apos;s user interface.</rdfs:comment>
    </owl:Class>
    


    <!-- http://purl.imsglobal.org/vocab/lti/v2/lti#IconStyle -->

    <owl:Class rdf:about="&lti;IconStyle">
        <rdfs:comment>&lt;p&gt;A resource that specifies the style for an Icon.&lt;/p&gt;
The LTI standard does not define any particular Icon styles.  Each vendor is free to publish its own set of icon styles.  A typical style might specify dimensions of the icon or its intended usage.  Each IconStyle is uniquely identified by a URI.  Ideally, the URI should resolve to a resource that provides a definition of the icon style.</rdfs:comment>
    </owl:Class>
    


    <!-- http://purl.imsglobal.org/vocab/lti/v2/lti#LocalizedName -->

    <owl:Class rdf:about="&lti;LocalizedName">
        <rdfs:subClassOf>
            <owl:Restriction>
                <owl:onProperty rdf:resource="&lti;default_value"/>
                <owl:allValuesFrom rdf:resource="&lti-type;LongName.Type"/>
            </owl:Restriction>
        </rdfs:subClassOf>
        <rdfs:comment>This container stores the default display name for some object plus a key that may be used to lookup a translation for the display name from a resource bundle for a particular locale.  The string value has a maximum length of 128 characters.</rdfs:comment>
    </owl:Class>
    


    <!-- http://purl.imsglobal.org/vocab/lti/v2/lti#LocalizedText -->

    <owl:Class rdf:about="&lti;LocalizedText">
        <rdfs:subClassOf>
            <owl:Restriction>
                <owl:onProperty rdf:resource="&lti;default_value"/>
                <owl:allValuesFrom rdf:resource="&lti-type;Text.Type"/>
            </owl:Restriction>
        </rdfs:subClassOf>
        <rdfs:comment>This container defines a block of text.  The container includes a default value for the text, plus a key that can be used to lookup a locale-specific value from a resource bundle.</rdfs:comment>
    </owl:Class>
    


    <!-- http://purl.imsglobal.org/vocab/lti/v2/lti#LtiLink -->

    <owl:Class rdf:about="&lti;LtiLink">
        <rdfs:subClassOf rdf:resource="&ci;ContentItem"/>
        <rdfs:subClassOf rdf:resource="&lti;ToolSettingsContainer"/>
        <rdfs:subClassOf>
            <owl:Restriction>
                <owl:onProperty rdf:resource="&lti;resource_link_id"/>
                <owl:minCardinality rdf:datatype="&xsd;nonNegativeInteger">1</owl:minCardinality>
            </owl:Restriction>
        </rdfs:subClassOf>
        <rdfs:comment>An &lt;code&gt;LtiLink&lt;/code&gt; represents a link within the Tool Consumer system pointing to a resource within the Tool Provider.</rdfs:comment>
    </owl:Class>
    


    <!-- http://purl.imsglobal.org/vocab/lti/v2/lti#MessageHandler -->

    <owl:Class rdf:about="&lti;MessageHandler">
        <rdfs:subClassOf rdf:resource="&lti;Endpoint"/>
        <rdfs:subClassOf>
            <owl:Restriction>
                <owl:onProperty rdf:resource="&lti;message_type"/>
                <owl:minCardinality rdf:datatype="&xsd;nonNegativeInteger">1</owl:minCardinality>
            </owl:Restriction>
        </rdfs:subClassOf>
        <rdfs:comment>Defines the features of a message handler, including information about the handler&apos;s service endpoint and custom parameters that it expects.</rdfs:comment>
    </owl:Class>
    


    <!-- http://purl.imsglobal.org/vocab/lti/v2/lti#MessageType -->

    <owl:Class rdf:about="&lti;MessageType">
        <rdfs:subClassOf rdf:resource="&lti;Capability"/>
        <rdfs:subClassOf>
            <owl:Restriction>
                <owl:onProperty rdf:resource="&lti;message_class"/>
                <owl:minCardinality rdf:datatype="&xsd;nonNegativeInteger">1</owl:minCardinality>
            </owl:Restriction>
        </rdfs:subClassOf>
        <rdfs:subClassOf>
            <owl:Restriction>
                <owl:onProperty rdf:resource="&lti;http_method"/>
                <owl:minCardinality rdf:datatype="&xsd;nonNegativeInteger">1</owl:minCardinality>
            </owl:Restriction>
        </rdfs:subClassOf>
        <rdfs:comment>This container holds metadata about a particular type of message.
It provides a friendly name (an alias) for the formal Message class name, and it specifies the allowed HTTP methods for Messages of the given type.</rdfs:comment>
    </owl:Class>
    


    <!-- http://purl.imsglobal.org/vocab/lti/v2/lti#Parameter -->

    <owl:Class rdf:about="&lti;Parameter">
        <rdfs:subClassOf>
            <owl:Restriction>
                <owl:onProperty rdf:resource="&lti;name"/>
                <owl:minCardinality rdf:datatype="&xsd;nonNegativeInteger">1</owl:minCardinality>
            </owl:Restriction>
        </rdfs:subClassOf>
        <rdfs:comment>Defines the characteristics of a parameter expected by a MessageHandler.</rdfs:comment>
    </owl:Class>
    


    <!-- http://purl.imsglobal.org/vocab/lti/v2/lti#ProductFamily -->

    <owl:Class rdf:about="&lti;ProductFamily">
        <rdfs:subClassOf rdf:resource="&lti;HasCode"/>
        <rdfs:subClassOf>
            <owl:Restriction>
                <owl:onProperty rdf:resource="&lti;vendor"/>
                <owl:minCardinality rdf:datatype="&xsd;nonNegativeInteger">1</owl:minCardinality>
            </owl:Restriction>
        </rdfs:subClassOf>
        <rdfs:comment>A ProductFamily represents the collection of all versions of a particular product over time.  Two products that have the same product &lt;em&gt;code&lt;/em&gt; belong to the same ProductFamily.  The LTI product model has four levels: &lt;OL&gt;
  &lt;LI&gt; &lt;code&gt;ProductFamily&lt;/code&gt;:  The collection of all versions of a given product.
  &lt;LI&gt; &lt;code&gt;ProductInfo&lt;/code&gt;: Encapsulates information about one particular version of a product.
  &lt;LI&gt; &lt;code&gt;ProductInstance&lt;/code&gt;: Represents one deployed instance of a particular version of a product.
  &lt;LI&gt; &lt;code&gt;ProductProfile&lt;/code&gt;: Defines a &lt;em&gt;view&lt;/em&gt; of a deployed instance of a product.  This view may be customized for different integration partners.
&lt;/OL&gt;

Notice that the ProductFamily sits at the top of the product hierarchy.  Each product family is owned by a &lt;code&gt;Vendor&lt;/code&gt;.</rdfs:comment>
    </owl:Class>
    


    <!-- http://purl.imsglobal.org/vocab/lti/v2/lti#ProductInfo -->

    <owl:Class rdf:about="&lti;ProductInfo">
        <rdfs:subClassOf>
            <owl:Restriction>
                <owl:onProperty rdf:resource="&lti;product_version"/>
                <owl:minCardinality rdf:datatype="&xsd;nonNegativeInteger">1</owl:minCardinality>
            </owl:Restriction>
        </rdfs:subClassOf>
        <rdfs:subClassOf>
            <owl:Restriction>
                <owl:onProperty rdf:resource="&lti;product_family"/>
                <owl:minCardinality rdf:datatype="&xsd;nonNegativeInteger">1</owl:minCardinality>
            </owl:Restriction>
        </rdfs:subClassOf>
        <rdfs:subClassOf>
            <owl:Restriction>
                <owl:onProperty rdf:resource="&lti;product_name"/>
                <owl:minCardinality rdf:datatype="&xsd;nonNegativeInteger">1</owl:minCardinality>
            </owl:Restriction>
        </rdfs:subClassOf>
        <rdfs:comment>Encapsulates information about one released version of a product (Tool Consumer or Tool).</rdfs:comment>
    </owl:Class>
    


    <!-- http://purl.imsglobal.org/vocab/lti/v2/lti#ProductInstance -->

    <owl:Class rdf:about="&lti;ProductInstance">
        <rdfs:subClassOf>
            <owl:Restriction>
                <owl:onProperty rdf:resource="&lti;guid"/>
                <owl:minCardinality rdf:datatype="&xsd;nonNegativeInteger">1</owl:minCardinality>
            </owl:Restriction>
        </rdfs:subClassOf>
        <rdfs:subClassOf>
            <owl:Restriction>
                <owl:onProperty rdf:resource="&lti;product_info"/>
                <owl:minCardinality rdf:datatype="&xsd;nonNegativeInteger">1</owl:minCardinality>
            </owl:Restriction>
        </rdfs:subClassOf>
        <rdfs:comment>The resource encapsulates information about one deployed instance of a web-based product (Tool or Tool Consumer).</rdfs:comment>
    </owl:Class>
    


    <!-- http://purl.imsglobal.org/vocab/lti/v2/lti#ProductProfile -->

    <owl:Class rdf:about="&lti;ProductProfile">
        <rdfs:subClassOf>
            <owl:Restriction>
                <owl:onProperty rdf:resource="&lti;product_instance"/>
                <owl:minCardinality rdf:datatype="&xsd;nonNegativeInteger">1</owl:minCardinality>
            </owl:Restriction>
        </rdfs:subClassOf>
        <rdfs:subClassOf>
            <owl:Restriction>
                <owl:onProperty rdf:resource="&lti;lti_version"/>
                <owl:allValuesFrom rdf:resource="&xsd;normalizedString"/>
            </owl:Restriction>
        </rdfs:subClassOf>
        <rdfs:comment>A ProductProfile presents an integration view of a deployed instance of some product (Tool or Tool Consumer).  It defines the services and other features offered to an integration partner.  A profile may be customized for each integration partner or shared with multiple partners.
&lt;p&gt;ProductProfile is the abstract base class for all product profiles. The ToolConsumerProfile and ToolProfile are derived from this base class.  &lt;/p&gt;</rdfs:comment>
    </owl:Class>
    


    <!-- http://purl.imsglobal.org/vocab/lti/v2/lti#PropertyMap -->

    <owl:Class rdf:about="&lti;PropertyMap">
        <rdfs:comment>An abstract class whose properties are defined by the Tool Provider and stored in the Tool Consumer.   When represented in JSON-LD, the PropertyMap object typically appears as a plain-old JSON object (though it may have a custom JSON-LD context that defines the semantics for the custom properties).  It is a best practice for the values in a PropertyMap to be strings.  This best practice may be revised if the development community expresses a desire to support other data types in a PropertyMap.</rdfs:comment>
    </owl:Class>
    


    <!-- http://purl.imsglobal.org/vocab/lti/v2/lti#ResourceHandler -->

    <owl:Class rdf:about="&lti;ResourceHandler">
        <rdfs:subClassOf>
            <owl:Restriction>
                <owl:onProperty rdf:resource="&lti;message"/>
                <owl:minCardinality rdf:datatype="&xsd;nonNegativeInteger">1</owl:minCardinality>
            </owl:Restriction>
        </rdfs:subClassOf>
        <rdfs:subClassOf>
            <owl:Restriction>
                <owl:onProperty rdf:resource="&lti;resource_type"/>
                <owl:minCardinality rdf:datatype="&xsd;nonNegativeInteger">1</owl:minCardinality>
            </owl:Restriction>
        </rdfs:subClassOf>
        <rdfs:subClassOf>
            <owl:Restriction>
                <owl:onProperty rdf:resource="&lti;resource_name"/>
                <owl:minCardinality rdf:datatype="&xsd;nonNegativeInteger">1</owl:minCardinality>
            </owl:Restriction>
        </rdfs:subClassOf>
        <rdfs:comment>The set of information for a specific resource handler.</rdfs:comment>
    </owl:Class>
    


    <!-- http://purl.imsglobal.org/vocab/lti/v2/lti#ResourceType -->

    <owl:Class rdf:about="&lti;ResourceType">
        <rdfs:subClassOf rdf:resource="&lti;HasCode"/>
        <rdfs:subClassOf>
            <owl:Restriction>
                <owl:onProperty rdf:resource="&lti;resource_type_owner"/>
                <owl:minCardinality rdf:datatype="&xsd;nonNegativeInteger">1</owl:minCardinality>
            </owl:Restriction>
        </rdfs:subClassOf>
        <rdfs:comment>This class represents all ResourceHandlers of a given type.  Two ResourceHandlers that belong to this set are considered to be different versions of the same ResourceHandler.</rdfs:comment>
    </owl:Class>
    


    <!-- http://purl.imsglobal.org/vocab/lti/v2/lti#RestService -->

    <owl:Class rdf:about="&lti;RestService">
        <rdfs:subClassOf rdf:resource="&lti;ServiceDescriptor"/>
        <rdfs:subClassOf>
            <owl:Restriction>
                <owl:onProperty rdf:resource="&lti;format"/>
                <owl:minCardinality rdf:datatype="&xsd;nonNegativeInteger">1</owl:minCardinality>
            </owl:Restriction>
        </rdfs:subClassOf>
        <rdfs:subClassOf>
            <owl:Restriction>
                <owl:onProperty rdf:resource="&lti;endpoint"/>
                <owl:minCardinality rdf:datatype="&xsd;nonNegativeInteger">1</owl:minCardinality>
            </owl:Restriction>
        </rdfs:subClassOf>
        <rdfs:subClassOf>
            <owl:Restriction>
                <owl:onProperty rdf:resource="&lti;action"/>
                <owl:minCardinality rdf:datatype="&xsd;nonNegativeInteger">1</owl:minCardinality>
            </owl:Restriction>
        </rdfs:subClassOf>
        <rdfs:comment>A descriptor for a REST service.</rdfs:comment>
    </owl:Class>
    


    <!-- http://purl.imsglobal.org/vocab/lti/v2/lti#RestServiceProfile -->

    <owl:Class rdf:about="&lti;RestServiceProfile">
        <rdfs:subClassOf rdf:resource="&lti;ServiceProfile"/>
        <rdfs:subClassOf>
            <owl:Restriction>
                <owl:onProperty rdf:resource="&lti;action"/>
                <owl:minCardinality rdf:datatype="&xsd;nonNegativeInteger">1</owl:minCardinality>
            </owl:Restriction>
        </rdfs:subClassOf>
        <rdfs:comment>A kind of ServiceProfile specialized for REST services. </rdfs:comment>
    </owl:Class>
    


    <!-- http://purl.imsglobal.org/vocab/lti/v2/lti#SecurityContract -->

    <owl:Class rdf:about="&lti;SecurityContract">
        <rdfs:subClassOf>
            <owl:Restriction>
                <owl:onProperty rdf:resource="&lti;shared_secret"/>
                <owl:minCardinality rdf:datatype="&xsd;nonNegativeInteger">1</owl:minCardinality>
            </owl:Restriction>
        </rdfs:subClassOf>
        <rdfs:comment>This entity specifies all aspects of the security agreements between Tool Provider and Tool Consumer.
&lt;p&gt;
Notice that the security contract distinguishes between &lt;code&gt;tool_service&lt;/code&gt;s and &lt;code&gt;end_user_service&lt;/code&gt;s.  A &lt;code&gt;tool_service&lt;/code&gt; is a service that the Tool invokes when acting on its own.  By contrast, a &lt;code&gt;end_user_service&lt;/code&gt; is a service that the Tool invokes when acting as an agent for some end user.  Consider, for example, the case where a Tool is reporting scores to the Tool Consumer via an outcomes service.  When a student submits an assignment, the Tool may calculate a score and post it to the Tool Consumer.  In this case the Tool is acting on its own since students generally do not have permission to enter their own scores into a grade book.  Now, suppose the Tool exposes a user interface which allows instructors to change a score.  In this case, when the Tool posts the modified score to the Tool Consumer grade book, it is acting as an agent for the end user.  This example, illustrates that the same service may be referenced as both a &lt;code&gt;tool_service&lt;/code&gt; and a &lt;code&gt;end_user_service&lt;/code&gt;
&lt;/p&gt;
</rdfs:comment>
    </owl:Class>
    


    <!-- http://purl.imsglobal.org/vocab/lti/v2/lti#ServiceDescriptor -->

    <owl:Class rdf:about="&lti;ServiceDescriptor">
        <rdfs:comment>This entity defines a profile for a service.  It is a &quot;profile&quot; in the sense that it specifies a subset of operations that are declared by the full  interface for some service.  For example, a profile might list the &quot;read&quot; operations of a service but exclude the &quot;write&quot; operations.  This is useful because a product (Tool or TC) might want to offer the read-only operations to a partner, but it might not want to expose write operations.  (On the other hand, it is perfectly legitimate for a profile to list all of the operations that are declared in the service interface if desired.)
ServiceProfiles are used for four different purposes: (1) they allow a product to advertise the operations that it offers to a partner, (2) they allow a product to declare the operations that it intends to use, (3) they allow a product to advertise the security profiles that are available for service operations, and (4) they allow a product to assert the security profiles that will be used for service operations. </rdfs:comment>
    </owl:Class>
    


    <!-- http://purl.imsglobal.org/vocab/lti/v2/lti#ServiceOwner -->

    <owl:Class rdf:about="&lti;ServiceOwner">
        <rdfs:subClassOf>
            <owl:Restriction>
                <owl:onProperty rdf:resource="&lti;timestamp"/>
                <owl:minCardinality rdf:datatype="&xsd;nonNegativeInteger">1</owl:minCardinality>
            </owl:Restriction>
        </rdfs:subClassOf>
        <rdfs:subClassOf>
            <owl:Restriction>
                <owl:onProperty rdf:resource="&lti;service_owner_name"/>
                <owl:minCardinality rdf:datatype="&xsd;nonNegativeInteger">1</owl:minCardinality>
            </owl:Restriction>
        </rdfs:subClassOf>
        <rdfs:comment>The entity that owns the services provided by a product instance.</rdfs:comment>
    </owl:Class>
    


    <!-- http://purl.imsglobal.org/vocab/lti/v2/lti#ServiceProfile -->

    <owl:Class rdf:about="&lti;ServiceProfile">
        <rdfs:subClassOf>
            <owl:Restriction>
                <owl:onProperty rdf:resource="&lti;service"/>
                <owl:minCardinality rdf:datatype="&xsd;nonNegativeInteger">1</owl:minCardinality>
            </owl:Restriction>
        </rdfs:subClassOf>
        <rdfs:comment>A profile for some service that may be invoked by an integration partner.  A profile specifies which methods or operations the integration partner intends to use.</rdfs:comment>
    </owl:Class>
    


    <!-- http://purl.imsglobal.org/vocab/lti/v2/lti#ServiceProvider -->

    <owl:Class rdf:about="&lti;ServiceProvider">
        <rdfs:subClassOf>
            <owl:Restriction>
                <owl:onProperty rdf:resource="&lti;guid"/>
                <owl:minCardinality rdf:datatype="&xsd;nonNegativeInteger">1</owl:minCardinality>
            </owl:Restriction>
        </rdfs:subClassOf>
        <rdfs:subClassOf>
            <owl:Restriction>
                <owl:onProperty rdf:resource="&lti;service_provider_name"/>
                <owl:minCardinality rdf:datatype="&xsd;nonNegativeInteger">1</owl:minCardinality>
            </owl:Restriction>
        </rdfs:subClassOf>
        <rdfs:subClassOf>
            <owl:Restriction>
                <owl:onProperty rdf:resource="&lti;timestamp"/>
                <owl:minCardinality rdf:datatype="&xsd;nonNegativeInteger">1</owl:minCardinality>
            </owl:Restriction>
        </rdfs:subClassOf>
        <rdfs:comment>This resource represents the service provider that hosts a product (Tool or Tool Consumer).</rdfs:comment>
    </owl:Class>
    


    <!-- http://purl.imsglobal.org/vocab/lti/v2/lti#ShortLocalizedName -->

    <owl:Class rdf:about="&lti;ShortLocalizedName">
        <rdfs:subClassOf>
            <owl:Restriction>
                <owl:onProperty rdf:resource="&lti;default_value"/>
                <owl:allValuesFrom rdf:resource="&lti-type;ShortName.Type"/>
            </owl:Restriction>
        </rdfs:subClassOf>
        <rdfs:comment>This container stores the default display name for some object plus a key that may be used to lookup a translation for the display name from a resource bundle for a particular locale.  This class is similar to LocalizedName, except that that the string value is limited to 64 characters.</rdfs:comment>
    </owl:Class>
    


    <!-- http://purl.imsglobal.org/vocab/lti/v2/lti#ToolConsumerProfile -->

    <owl:Class rdf:about="&lti;ToolConsumerProfile">
        <rdfs:subClassOf rdf:resource="&lti;ProductProfile"/>
        <rdfs:subClassOf>
            <owl:Restriction>
                <owl:onProperty rdf:resource="&lti;guid"/>
                <owl:minCardinality rdf:datatype="&xsd;nonNegativeInteger">1</owl:minCardinality>
            </owl:Restriction>
        </rdfs:subClassOf>
        <rdfs:comment>The profile for a Tool Consumer product.</rdfs:comment>
    </owl:Class>
    


    <!-- http://purl.imsglobal.org/vocab/lti/v2/lti#ToolProfile -->

    <owl:Class rdf:about="&lti;ToolProfile">
        <rdfs:subClassOf rdf:resource="&lti;ProductProfile"/>
        <rdfs:subClassOf>
            <owl:Restriction>
                <owl:onProperty rdf:resource="&lti;base_url_choice"/>
                <owl:minCardinality rdf:datatype="&xsd;nonNegativeInteger">1</owl:minCardinality>
            </owl:Restriction>
        </rdfs:subClassOf>
        <rdfs:comment>The profile for a Tool product.</rdfs:comment>
    </owl:Class>
    


    <!-- http://purl.imsglobal.org/vocab/lti/v2/lti#ToolProxy -->

    <owl:Class rdf:about="&lti;ToolProxy">
        <rdfs:subClassOf rdf:resource="&lti;ToolSettingsContainer"/>
        <rdfs:subClassOf>
            <owl:Restriction>
                <owl:onProperty rdf:resource="&lti;tool_profile"/>
                <owl:minCardinality rdf:datatype="&xsd;nonNegativeInteger">1</owl:minCardinality>
            </owl:Restriction>
        </rdfs:subClassOf>
        <rdfs:subClassOf>
            <owl:Restriction>
                <owl:onProperty rdf:resource="&lti;tool_proxy_guid"/>
                <owl:minCardinality rdf:datatype="&xsd;nonNegativeInteger">1</owl:minCardinality>
            </owl:Restriction>
        </rdfs:subClassOf>
        <rdfs:subClassOf>
            <owl:Restriction>
                <owl:onProperty rdf:resource="&lti;tool_consumer_profile"/>
                <owl:minCardinality rdf:datatype="&xsd;nonNegativeInteger">1</owl:minCardinality>
            </owl:Restriction>
        </rdfs:subClassOf>
        <rdfs:subClassOf>
            <owl:Restriction>
                <owl:onProperty rdf:resource="&lti;lti_version"/>
                <owl:allValuesFrom rdf:resource="&xsd;token"/>
            </owl:Restriction>
        </rdfs:subClassOf>
        <rdfs:subClassOf>
            <owl:Restriction>
                <owl:onProperty rdf:resource="&lti;security_contract"/>
                <owl:minCardinality rdf:datatype="&xsd;nonNegativeInteger">1</owl:minCardinality>
            </owl:Restriction>
        </rdfs:subClassOf>
        <rdfs:comment>This entity defines the integration contract between a ToolConsumer and a Tool.   It is called a &quot;ToolProxy&quot; because its primary purpose is to provide the ToolConsumer with all of the information needed to embed a given Tool within the ToolConsumer system.</rdfs:comment>
    </owl:Class>
    


    <!-- http://purl.imsglobal.org/vocab/lti/v2/lti#ToolProxyBinding -->

    <owl:Class rdf:about="&lti;ToolProxyBinding">
        <rdfs:subClassOf rdf:resource="&lti;ToolSettingsContainer"/>
        <rdfs:subClassOf>
            <owl:Restriction>
                <owl:onProperty rdf:resource="&lti;context"/>
                <owl:minCardinality rdf:datatype="&xsd;nonNegativeInteger">1</owl:minCardinality>
            </owl:Restriction>
        </rdfs:subClassOf>
        <rdfs:comment>A &lt;code&gt;ToolProxyBinding&lt;/code&gt; associates a ToolProxy with a learning Context (such as a Course Section).   This association must be established before the corresponding Tool can be used within the Context.  The &lt;code&gt;ToolProxyBinding&lt;/code&gt; also serves as a container that holds tool settings associated with the learning Context.</rdfs:comment>
    </owl:Class>
    


    <!-- http://purl.imsglobal.org/vocab/lti/v2/lti#ToolSettingsContainer -->

    <owl:Class rdf:about="&lti;ToolSettingsContainer">
        <rdfs:comment>&lt;code&gt;ToolSettingsContainer&lt;/code&gt; is the base class for all resources that encapsulate tool settings.</rdfs:comment>
    </owl:Class>
    


    <!-- http://purl.imsglobal.org/vocab/lti/v2/lti#Vendor -->

    <owl:Class rdf:about="&lti;Vendor">
        <rdfs:subClassOf rdf:resource="&lti;HasCode"/>
        <rdfs:subClassOf>
            <owl:Restriction>
                <owl:onProperty rdf:resource="&lti;timestamp"/>
                <owl:minCardinality rdf:datatype="&xsd;nonNegativeInteger">1</owl:minCardinality>
            </owl:Restriction>
        </rdfs:subClassOf>
        <rdfs:subClassOf>
            <owl:Restriction>
                <owl:onProperty rdf:resource="&lti;vendor_name"/>
                <owl:minCardinality rdf:datatype="&xsd;nonNegativeInteger">1</owl:minCardinality>
            </owl:Restriction>
        </rdfs:subClassOf>
        <rdfs:comment>A person or agency that offers products to the market. The key types of products relevant to LTI are Tools (which are described by Tool Profiles) and Tool Consumers (which are described by Tool Consumer Profiles).</rdfs:comment>
    </owl:Class>
    


    <!-- http://purl.imsglobal.org/xsd/lti/v2/ltid#DataValue.Type -->

    <owl:Class rdf:about="&lti-type;DataValue.Type"/>
    


    <!-- http://purl.imsglobal.org/xsd/lti/v2/ltid#GUID.Type -->

    <owl:Class rdf:about="&lti-type;GUID.Type"/>
    


    <!-- http://purl.imsglobal.org/xsd/lti/v2/ltid#LongName.Type -->

    <owl:Class rdf:about="&lti-type;LongName.Type"/>
    


    <!-- http://purl.imsglobal.org/xsd/lti/v2/ltid#Name.Type -->

    <owl:Class rdf:about="&lti-type;Name.Type"/>
    


    <!-- http://purl.imsglobal.org/xsd/lti/v2/ltid#ShortName.Type -->

    <owl:Class rdf:about="&lti-type;ShortName.Type"/>
    


    <!-- http://purl.imsglobal.org/xsd/lti/v2/ltid#Text.Type -->

    <owl:Class rdf:about="&lti-type;Text.Type"/>
    


    <!-- http://purl.imsglobal.org/xsd/lti/v2/ltid#Token.Type -->

    <owl:Class rdf:about="&lti-type;Token.Type"/>
    


    <!-- http://purl.imsglobal.org/xsd/lti/v2/ltid#VariableName.Type -->

    <owl:Class rdf:about="&lti-type;VariableName.Type"/>
    


    <!-- http://purl.org/semantictools/v1/vocab/bind#TargetNamespace -->

    <owl:Class rdf:about="&bind;TargetNamespace"/>
    


    <!-- http://www.w3.org/2001/XMLSchema#normalizedString -->

    <owl:Class rdf:about="&xsd;normalizedString"/>
    


    <!-- http://www.w3.org/2001/XMLSchema#token -->

    <owl:Class rdf:about="&xsd;token"/>
    


    <!-- http://www.w3.org/2002/07/owl#Class -->

    <owl:Class rdf:about="&owl;Class"/>
    


    <!-- 
    ///////////////////////////////////////////////////////////////////////////////////////
    //
    // Individuals
    //
    ///////////////////////////////////////////////////////////////////////////////////////
     -->

    


    <!-- http://purl.imsglobal.org/vocab/lti/v2/lti# -->

    <owl:NamedIndividual rdf:about="http://purl.imsglobal.org/vocab/lti/v2/lti#">
        <rdf:type rdf:resource="&bind;TargetNamespace"/>
    </owl:NamedIndividual>
    


    <!-- http://purl.imsglobal.org/vocab/lti/v2/lti#GET -->

    <owl:NamedIndividual rdf:about="&lti;GET"/>
    


    <!-- http://purl.imsglobal.org/vocab/lti/v2/lti#POST -->

    <owl:NamedIndividual rdf:about="&lti;POST"/>
    


    <!-- http://purl.imsglobal.org/vocab/lti/v2/lti#embed -->

    <owl:NamedIndividual rdf:about="&lti;embed">
        <rdf:type rdf:resource="&lti;DocumentTarget"/>
    </owl:NamedIndividual>
    


    <!-- http://purl.imsglobal.org/vocab/lti/v2/lti#frame -->

    <owl:NamedIndividual rdf:about="&lti;frame">
        <rdf:type rdf:resource="&lti;DocumentTarget"/>
    </owl:NamedIndividual>
    


    <!-- http://purl.imsglobal.org/vocab/lti/v2/lti#iframe -->

    <owl:NamedIndividual rdf:about="&lti;iframe">
        <rdf:type rdf:resource="&lti;DocumentTarget"/>
    </owl:NamedIndividual>
    


    <!-- http://purl.imsglobal.org/vocab/lti/v2/lti#overlay -->

    <owl:NamedIndividual rdf:about="&lti;overlay">
        <rdf:type rdf:resource="&lti;DocumentTarget"/>
    </owl:NamedIndividual>
    


    <!-- http://purl.imsglobal.org/vocab/lti/v2/lti#popup -->

    <owl:NamedIndividual rdf:about="&lti;popup">
        <rdf:type rdf:resource="&lti;DocumentTarget"/>
    </owl:NamedIndividual>
    


    <!-- http://purl.imsglobal.org/vocab/lti/v2/lti#window -->

    <owl:NamedIndividual rdf:about="&lti;window">
        <rdf:type rdf:resource="&lti;DocumentTarget"/>
    </owl:NamedIndividual>
    <rdf:Description>
        <rdfs:comment>This is a human-readable description of the Vendor.</rdfs:comment>
    </rdf:Description>
    <rdf:Description>
        <rdfs:comment>Defines a human readable name for the Vendor.  The name should be suitable for display in management screens within the Tool Provider system.</rdfs:comment>
    </rdf:Description>
    <rdf:Description>
        <rdfs:comment>A timestamp for the Vendor record. This value is useful for determining which record is most current.</rdfs:comment>
    </rdf:Description>
    <rdf:Description>
        <rdfs:comment>The default value for the display name.  This value is used if (1) the key attribute is undefined, (2) the localization capability is not enabled, or (3) a value for the specified key is not found in the locale-specific resource bundle.</rdfs:comment>
    </rdf:Description>
    <rdf:Description>
        <rdfs:comment>&lt;p&gt;A group of related products offered by the Vendor.  All of the products within a given product family are different &lt;em&gt;versions&lt;/em&gt; of the same product. &lt;/p&gt;
&lt;p&gt;A vendor may have multiple product families.  For example, the same vendor might offer a discussion forum tool and also a white board tool.  Each of these tools corresponds to a different product family.&lt;/p&gt;</rdfs:comment>
    </rdf:Description>
    <rdf:Description>
        <rdfs:comment>This is the URL of the vendor.</rdfs:comment>
    </rdf:Description>
    <rdf:Description>
        <rdfs:comment>An inverse attribute which references the ProductInstance within which this ProductProfile is defined.</rdfs:comment>
    </rdf:Description>
    <rdf:Description>
        <rdfs:comment>The descriptor for a service offered by the product (Tool or Tool Consumer).</rdfs:comment>
    </rdf:Description>
    <rdf:Description>
        <rdfs:comment>The identifier for an LTI version that the version supports.  A given product (Tool or Tool Consumer) may support multiple versions, but only one version is selected for use in the integration contract.</rdfs:comment>
    </rdf:Description>
    <rdf:Description>
        <rdfs:comment>A collection of custom properties defined by the Tool Provider and stored in this ToolSettingsContainer.</rdfs:comment>
    </rdf:Description>
    <rdf:Description>
        <rdfs:comment>The name of the resource handler suitable for display in the TC user interface.</rdfs:comment>
    </rdf:Description>
    <rdf:Description>
        <rdfs:comment>The REST endpoint at which custom tool settings may be accessed for this ToolSettingsContainer.</rdfs:comment>
    </rdf:Description>
    <rdf:Description>
        <rdfs:comment>A capability offered by the Tool Consumer to its integration partners.</rdfs:comment>
    </rdf:Description>
    <rdf:Description>
        <rdfs:comment>A LineItem that records results for some learning activity within this context.</rdfs:comment>
    </rdf:Description>
    <rdf:Description>
        <rdfs:comment>Provides information about a graphical icon that represents the resource described by this ResourceHandler.</rdfs:comment>
    </rdf:Description>
    <rdf:Description>
        <rdfs:comment>Identifies the type of resource associated with this ResourceHandler.  Resource types are identified by a code that is unique within a given ProductFamily.</rdfs:comment>
    </rdf:Description>
    <rdf:Description>
        <rdfs:comment>Defines the features of a message handler associated with the resource described by this ResourceHandler.</rdfs:comment>
    </rdf:Description>
    <rdf:Description>
        <rdfs:comment>Denotes that the parameter has a variable value that is automatically substituted at run-time.  The value of this attribute is the name for a variable whose value will be added to the message at run-time. </rdfs:comment>
    </rdf:Description>
    <rdf:Description>
        <rdfs:comment>The key used to lookup the locale-specific value from a resource bundle.</rdfs:comment>
    </rdf:Description>
    <rdf:Description>
        <rdfs:comment>The name of the parameter.</rdfs:comment>
    </rdf:Description>
    <rdf:Description>
        <rdfs:comment>Denotes that the value of the parameter is fixed at the time of definition within the product profile.  This value must be passed in each message of the associated message type.</rdfs:comment>
    </rdf:Description>
    <rdf:Description>
        <rdfs:comment>The profile for a Tool Consumer service that may be invoked by the Tool when acting as an agent for some end user.  </rdfs:comment>
    </rdf:Description>
    <rdf:Description>
        <rdfs:comment>The profile for a Tool Consumer service that may be invoked by the Tool acting on its own (as opposed to acting as an agent for some end user).  </rdfs:comment>
    </rdf:Description>
    <rdf:Description>
        <rdfs:comment>Specifies an HTTP method (POST, GET, PUT, etc.) which the integration partner intends to use.   A RestServiceProfile may include more than one action.  However, the set of actions declared in a RestServiceProfile must be a subset of actions declared in the RestService referenced by the &lt;code&gt;service&lt;/code&gt; property.</rdfs:comment>
    </rdf:Description>
    <rdf:Description>
        <rdfs:comment>The descriptor for the service that is being profiled.</rdfs:comment>
    </rdf:Description>
    <rdf:Description>
        <rdfs:comment>Specifies a custom parameter that is expected by the MessageHandler.</rdfs:comment>
    </rdf:Description>
    <rdf:Description>
        <rdfs:comment>The type of message that can be submitted to the Message Handler.</rdfs:comment>
    </rdf:Description>
    <rdf:Description>
        <rdfs:comment>A name for the product, suitable for display to end users.</rdfs:comment>
    </rdf:Description>
    <rdf:Description>
        <rdfs:comment>This is the version of the product. </rdfs:comment>
    </rdf:Description>
    <rdf:Description>
        <rdfs:comment>This is a description of the product suitable for display to end-users.</rdfs:comment>
    </rdf:Description>
    <rdf:Description>
        <rdfs:comment>This is a human readable description of the technical aspects of this product that might be of interest to developers who wish to integrate with this product via LTI.</rdfs:comment>
    </rdf:Description>
    <rdf:Description>
        <rdfs:comment>An inverse attribute that references the ProductFamily within which this ProductInfo is defined.</rdfs:comment>
    </rdf:Description>
    <rdf:Description>
        <rdfs:comment>A deployed instance of a particular version of a product (Tool or Tool Consumer).</rdfs:comment>
    </rdf:Description>
    <rdf:Description>
        <rdfs:comment>The vendor that owns the ProductFamily.</rdfs:comment>
    </rdf:Description>
    <rdf:Description>
        <rdfs:comment>Encapsulates information about one version of the product.</rdfs:comment>
    </rdf:Description>
    <rdf:Description>
        <rdfs:comment>Contact information for this Vendor.</rdfs:comment>
    </rdf:Description>
    <rdf:Description>
        <rdfs:comment>Specifies whether the path for this message type is allowed to be specified using an absolute path.  A value of &quot;false&quot; means that the MessageHandler must declare a relative path.</rdfs:comment>
    </rdf:Description>
    <rdf:Description>
        <rdfs:comment>This attribute identifies the formal Class definition the type of message that can be delivered to a given MessageHandler.</rdfs:comment>
    </rdf:Description>
    <rdf:Description>
        <rdfs:comment>Specifies an HTTP method (POST, GET, PUT, etc.) for the type of messages represented by this MessageType.</rdfs:comment>
    </rdf:Description>
    <rdf:Description>
        <rdfs:comment>This is the shared secret used for communications between the Tool Consumer and the Tool Provider.  It is expected that the Tool Consumer present an interface to the administrative user for them to activate the Tool Proxy before this secret is ever used by the Tool Consumer. 
The shared secret may be updated when a tool is re-registered (see the reregisterTool operation of the ToolRegistrationService).  In addition, the TC and TP should provide interfaces which allow their respective administrators to change the shared secret through an out-of-band agreement.</rdfs:comment>
    </rdf:Description>
    <rdf:Description>
        <rdfs:comment>A timestamp for the ServiceProvider record. This value is useful for determining which record is most current.</rdfs:comment>
    </rdf:Description>
    <rdf:Description>
        <rdfs:comment>The name of the service provider, suitable for display to end users.</rdfs:comment>
    </rdf:Description>
    <rdf:Description>
        <rdfs:comment>The entity that owns the services provided by this product instance.</rdfs:comment>
    </rdf:Description>
    <rdf:Description>
        <rdfs:comment>Contact information for support on this deployed instance of the product (Tool or ToolConsumer).</rdfs:comment>
    </rdf:Description>
    <rdf:Description>
        <rdfs:comment>A resource that presents a view of this ProductInstance to one or more integration partners.</rdfs:comment>
    </rdf:Description>
    <rdf:Description>
        <rdfs:comment>This is metadata about the product described in the profile.</rdfs:comment>
    </rdf:Description>
    <rdf:Description>
        <rdfs:comment>A description of the service provider, suitable for display to end-users.</rdfs:comment>
    </rdf:Description>
    <rdf:Description>
        <rdfs:comment>This is the base URL that should be used by default for all entities specified by the associated BaseUrlSelector.  The secure_base_url attribute may override this default Base URL.</rdfs:comment>
    </rdf:Description>
    <rdf:Description>
        <rdfs:comment>This is the base URL that should be used whenever security is enabled.  If this base URL is not defined, then the default_base_url is used in all circumstances.</rdfs:comment>
    </rdf:Description>
    <rdf:Description>
        <rdfs:comment>A resource that specifies the objects to which this BaseUrlChoice applies. </rdfs:comment>
    </rdf:Description>
    <rdf:Description>
        <rdfs:comment>The class of resources selected by this BaseUrlSelector.</rdfs:comment>
    </rdf:Description>
    <rdf:Description>
        <rdfs:comment>The email of the primary contact for the associated object.</rdfs:comment>
    </rdf:Description>
    <rdf:Description>
        <rdfs:comment>This attribute specifies the path for an endpoint such as a MessageHandler or an Icon. Typically, this path is relative to one of the base URL values defined in a BaseUrlChoice.  
In the case of a MessageHandler, the path may be an absolute path if the associated message type explicitly declares that an absolute path is allowed.  </rdfs:comment>
    </rdf:Description>
    <rdf:Description>
        <rdfs:comment>A globally unique identifier for the service provider.  As a best practice, this value should match an Internet domain name assigned by ICANN, but any globally unique identifier is acceptable.  </rdfs:comment>
    </rdf:Description>
    <rdf:Description>
        <rdfs:comment>If localization is supported then the key identifies a property in the bundle returned by the get-bundle-request message handler. </rdfs:comment>
    </rdf:Description>
    <rdf:Description>
        <rdfs:comment>This is the default value for the text. This default value  is used if (1) the key is not specified, (2) the localization capability is not enabled, or (3) the specified key is not found in the locale-specific resource bundle.</rdfs:comment>
    </rdf:Description>
    <rdf:Description>
        <rdfs:comment>The key used to lookup the locale-specific value from a resource bundle.</rdfs:comment>
    </rdf:Description>
    <rdf:Description>
        <rdfs:comment>The default value for the display name.  This value is used if (1) the key attribute is undefined, (2) the localization capability is not enabled, or (3) a value for the specified key is not found in the locale-specific resource bundle.</rdfs:comment>
    </rdf:Description>
    <rdf:Description>
        <rdfs:comment>Specifies the default path to an icon.  The absolute URL is formed by appending this path to the appropriate base URL for icons.</rdfs:comment>
    </rdf:Description>
    <rdf:Description>
        <rdfs:comment>The style of the icon referenced by this IconInfo.</rdfs:comment>
    </rdf:Description>
    <rdf:Description>
        <rdfs:comment>Contact information for support from a service provider.</rdfs:comment>
    </rdf:Description>
    <rdf:Description>
        <rdfs:comment>If localization is supported then the &apos;key&apos; attribute identifies a property in the resource bundle provided in response to the get-bundle-request message. The value of that property is the locale-specific path to the icon.</rdfs:comment>
    </rdf:Description>
    <rdf:Description>
        <rdfs:comment>This is the service provider that hosts the deployed product.</rdfs:comment>
    </rdf:Description>
    <rdf:Description>
        <rdfs:comment>A URI template that defines the REST endpoint for resources that may be accessed via the REST service.  The URI template should conform to the syntax in the proposed IETF standard [&lt;a href=&quot;http://www.ietf.org/id/draft-gregorio-uritemplate-08.txt&quot;&gt;draft-gregorio-uritemplate-08&lt;/a&gt;]. </rdfs:comment>
    </rdf:Description>
    <rdf:Description>
        <rdfs:comment>Specifies an HTTP action that is supported at the REST endpoint.  A given endpoint may support more than one action.  For example, it is common practice for a collection endpoint to accept POST requests, and a different item endpoint to accept GET, PUT, and DELETE requests.</rdfs:comment>
    </rdf:Description>
    <rdf:Description>
        <rdfs:comment>A unique identifier for the resource.</rdfs:comment>
    </rdf:Description>
    <rdf:Description>
        <rdfs:comment>The content type (also known as media type) of resources accessed via the endpoint defined by this RestService descriptor.   The endpoint of a REST service may support more than one content type if content negotiation is enabled as described in the &lt;a href=&quot;http://www.w3.org/Protocols/rfc2616/rfc2616-sec12.html&quot;&gt;HTTP 1.1&lt;/a&gt; specification.</rdfs:comment>
    </rdf:Description>
    <rdf:Description>
        <rdfs:comment>A capability that is enabled for messages handled by this MessageHandler.</rdfs:comment>
    </rdf:Description>
    <rdf:Description>
        <rdfs:comment>A globally unique identifier for this LTI link.</rdfs:comment>
    </rdf:Description>
    <rdf:Description>
        <rdfs:comment>The learning Context associated with this &lt;code&gt;ToolProxyBinding&lt;/code&gt;.</rdfs:comment>
    </rdf:Description>
    <rdf:Description>
        <rdfs:comment>A unique string provided by the tool consumer to identify the context (as passed in the context_id launch parameter).</rdfs:comment>
    </rdf:Description>
    <rdf:Description>
        <rdfs:comment>The globally unique identifier for the ToolProxy (a.k.a. integration contract).</rdfs:comment>
    </rdf:Description>
    <rdf:Description>
        <rdfs:comment>The profile of the Tool that is participating in the integration governed by this ToolProxy.</rdfs:comment>
    </rdf:Description>
    <rdf:Description>
        <rdfs:comment>The security aspect of an integration contract between two parties.</rdfs:comment>
    </rdf:Description>
    <rdf:Description>
        <rdfs:comment>The profile of the Tool Consumer that is participating in the integration governed by this ToolProxy.</rdfs:comment>
    </rdf:Description>
    <rdf:Description>
        <rdfs:comment>The LTI version that governs the integration between the Tool and ToolConsumer. </rdfs:comment>
    </rdf:Description>
</rdf:RDF>



<!-- Generated by the OWL API (version 3.5.0) http://owlapi.sourceforge.net -->

