@prefix ldp: <http://www.w3.org/ns/ldp#> .
@prefix rdfs: <http://www.w3.org/2000/01/rdf-schema#> .
@prefix rdf: <http://www.w3.org/1999/02/22-rdf-syntax-ns#> .
@prefix owl: <http://www.w3.org/2002/07/owl#> .
@prefix xsd: <http://www.w3.org/2001/XMLSchema#> .
@prefix bind: <http://purl.org/semantictools/v1/vocab/bind#> .

<http://www.w3.org/ns/ldp#> a owl:Ontology  ;
  rdfs:label "W3C Linked Data Platform" ;
  a bind:TargetNamespace ;
  bind:suggestedPrefix "ldp" .

ldp:Container rdf:type owl:Class;
  rdfs:subClassOf 
  [ a owl:Restriction ;
    owl:onProperty      ldp:membershipSubject;
    owl:minCardinality  1;
    rdfs:comment "Indicates which resource is the subject for the members of the container."
  ] ,
  [ a owl:Restriction ;
    owl:onProperty      ldp:membershipPredicate;
    owl:minCardinality  1;
    rdfs:comment "Indicates which predicate of the container's subject should be used to determine membership in the container."
  ] ; 
  rdfs:comment "A container that holds a collection of resources.  New resources are added to the container by submitting an HTTP POST request to the container endpoint. " .

ldp:Page rdf:type owl:Class;
  rdfs:subClassOf 
  [ a owl:Restriction ;
    owl:onProperty      ldp:pageOf;
    owl:minCardinality  1;
    rdfs:comment "Associates a page with its container."
  ] ,
  [ a owl:Restriction ;
    owl:onProperty      ldp:nextPage;
    owl:minCardinality  1
  ] ; 
  rdfs:comment "A resource that represents a limited set of members of a LDP Container." .

ldp:membershipSubject rdf:type owl:FunctionalProperty ;
  rdfs:domain ldp:Container ;
  rdfs:range rdfs:Resource ;
  rdfs:comment "Indicates which resource is the subject for the members of the container." .

ldp:membershipPredicate rdf:type owl:FunctionalProperty ;
  rdfs:domain ldp:Container ;
  rdfs:range rdf:Property ;
  rdfs:comment "Indicates which predicate of the container's subject should be used to determine membership in the container." .

ldp:pageOf rdf:type owl:FunctionalProperty ;
  rdfs:domain ldp:Page ;
  rdfs:range ldp:Container ;
  rdfs:comment "Associates a page with its container." .

ldp:nextPage rdf:type owl:FunctionalProperty ;
  rdfs:domain ldp:Page ;
  rdfs:range ldp:Page .

